formal/inference/Learn_EFSM.thy
@@ -4,33 +4,19 @@ begin
 
 declare One_nat_def [simp del]
 
-definition selectCoke :: transition where
-  "selectCoke = \<lparr>Label = (STR ''select''), Arity = 1, Guard = [gexp.Eq (V (I 1)) (L ((Str ''coke'')))], Outputs = [], Updates = []\<rparr>"
+abbreviation "coke \<equiv> STR ''coke''"
+abbreviation "pepsi \<equiv> STR ''pepsi''"
+abbreviation "beer \<equiv> STR ''beer''"
 
-definition coin50_50 :: transition where
-  "coin50_50 = \<lparr>Label = (STR ''coin''), Arity = 1, Guard = [gexp.Eq (V (I 1)) (L (Num 50))], Outputs = [L (Num 50)], Updates = []\<rparr>"
+abbreviation "coin i out \<equiv> \<lparr>Label = STR ''coin'', Arity = 1, Guard = [gexp.Eq (V (I (1))) (L (Num i))], Outputs = [L (Num out)], Updates = []\<rparr>"
+abbreviation "select i \<equiv> \<lparr>Label = STR ''select'', Arity = 1, Guard = [gexp.Eq (V (I 1)) (L (Value.Str i))], Outputs = [], Updates = []\<rparr>"
+abbreviation "vend out \<equiv> \<lparr>Label = STR ''vend'', Arity = 0, Guard = [], Outputs = [L (Value.Str out)], Updates = []\<rparr>"
 
-definition coin50_100 :: transition where
-  "coin50_100 = \<lparr>Label = (STR ''coin''), Arity = 1, Guard = [gexp.Eq (V (I 1)) (L (Num 50))], Outputs = [L (Num 100)], Updates = []\<rparr>"
-
-definition vend_coke :: transition where
-  "vend_coke = \<lparr>Label = (STR ''vend''), Arity = 0, Guard = [], Outputs = [L ((Str ''coke''))], Updates = []\<rparr>"
-
-definition coin100_100 :: transition where
-  "coin100_100 = \<lparr>Label = (STR ''coin''), Arity = 1, Guard = [gexp.Eq (V (I 1)) (L (Num 100))], Outputs = [L (Num 100)], Updates = []\<rparr>"
-
-definition selectPepsi :: transition where
-  "selectPepsi = \<lparr>Label = (STR ''select''), Arity = 1, Guard = [gexp.Eq (V (I 1)) (L ((Str ''pepsi'')))], Outputs = [], Updates = []\<rparr>"
-
-definition vend_pepsi :: transition where
-  "vend_pepsi = \<lparr>Label = (STR ''vend''), Arity = 0, Guard = [], Outputs = [L ((Str ''pepsi''))], Updates = []\<rparr>"
-
-lemmas transitions = selectCoke_def coin50_50_def coin50_100_def vend_coke_def selectPepsi_def coin100_100_def vend_pepsi_def
 
 definition pta :: iEFSM where
-  "pta = {|(0, (0, 1), selectCoke),  (2, (1, 2), coin50_50), (4, (2, 3), coin50_100),  (5, (3, 4), vend_coke),
-                                                             (3, (1, 5), coin100_100), (6, (5, 6), vend_coke),
-           (1, (0, 7), selectPepsi), (7, (7, 8), coin50_50), (8, (8, 9), coin50_100),  (9, (9, 10), vend_pepsi)|}"
+  "pta = {|(0, (0, 1), select coke),  (2, (1, 2), coin 50 50), (4, (2, 3), coin 50 100),  (5, (3, 4), (vend coke)),
+                                                             (3, (1, 5), coin 100 100), (6, (5, 6), (vend coke)),
+           (1, (0, 7), select pepsi), (7, (7, 8), coin 50 50), (8, (8, 9), coin 50 100),  (9, (9, 10), (vend pepsi))|}"
 
 lemma implode_pepsi: "String.implode ''pepsi'' = STR ''pepsi''"
   by (metis Literal.rep_eq String.implode_explode_eq zero_literal.rep_eq)
@@ -50,273 +36,11 @@ lemma explode_coke: "String.explode (STR ''coke'') = ''coke''"
 lemma explode_pepsi: "String.explode (STR ''pepsi'') = ''pepsi''"
   by (simp add: Literal.rep_eq zero_literal.rep_eq)
 
-lemma step_pta_selectPepsi: "step (tm pta) 0 Map.empty (STR ''select'') [(Str ''pepsi'')] = Some (selectPepsi, 7, [], <>)"
-proof-
-  have possible_steps: "possible_steps (tm pta) 0 Map.empty (STR ''select'') [(Str ''pepsi'')] = {|(7, selectPepsi)|}"
-    apply (simp add: possible_steps_def ffilter_def fimage_def fset_both_sides Abs_fset_inverse)
-    apply (simp add: tm_def pta_def Set.filter_def)
-    apply safe
-                      apply (simp_all add: transitions implode_coke implode_pepsi)
-    using Str_pepsi by force
-  show ?thesis
-    apply (simp add: step_def possible_steps)
-    by (simp add: selectPepsi_def)
-qed
-
 definition traces :: log where
   "traces = [[((STR ''select''), [(Str ''coke'')], []), ((STR ''coin''), [Num 50], [Num 50]), ((STR ''coin''), [Num 50], [Num 100]), ((STR ''vend''), [], [(Str ''coke'')])],
              [((STR ''select''), [(Str ''coke'')], []), ((STR ''coin''), [Num 100], [Num 100]), ((STR ''vend''), [], [(Str ''coke'')])],
              [((STR ''select''), [(Str ''pepsi'')], []), ((STR ''coin''), [Num 50], [Num 50]), ((STR ''coin''), [Num 50], [Num 100]), ((STR ''vend''), [], [(Str ''pepsi'')])]]"
 
-
-lemma build_pta: "toiEFSM (make_pta traces {||}) = pta"
-proof-
- have step_coin50: "step {|((0, 1), \<lparr>Label = (STR ''select''), Arity = Suc 0, Guard = [gexp.Eq (V (I 1)) (L ((Str ''coke'')))], Outputs = [], Updates = []\<rparr>)|} 1 Map.empty
-           (STR ''coin'') [Num 50] = None"
-    proof-
-      have set_filter: "(Set.filter
-         (\<lambda>((origin, dest), t).
-             origin = 1 \<and>
-             Label t = (STR ''coin'') \<and>
-             Suc 0 = Arity t \<and> apply_guards (Guard t) (case_vname (\<lambda>n. if n = 1 then Some (Num 50) else input2state [] (1 + 1) (I n)) Map.empty))
-         {((0, 1), \<lparr>Label = (STR ''select''), Arity = Suc 0, Guard = [gexp.Eq (V (I 1)) (L ((Str ''coke'')))], Outputs = [], Updates = []\<rparr>)}) = {}"
-        by (simp add: Set.filter_def)
-      show ?thesis
-        by (simp add: step_def possible_steps_def ffilter_def set_filter)
-    qed
-    have step_coin50_2: "step
-           {|((1, 2), \<lparr>Label = (STR ''coin''), Arity = Suc 0, Guard = [gexp.Eq (V (I 1)) (L (Num 50))], Outputs = [L (Num 50)], Updates = []\<rparr>),
-             ((0, 1), \<lparr>Label = (STR ''select''), Arity = Suc 0, Guard = [gexp.Eq (V (I 1)) (L ((Str ''coke'')))], Outputs = [], Updates = []\<rparr>)|}
-           2 Map.empty (STR ''coin'') [Num 50] = None"
-    proof-
-      have set_filter: "Set.filter
-         (\<lambda>((origin, dest), t).
-             origin = (2::nat) \<and>
-             Label t = (STR ''coin'') \<and>
-             Suc 0 = Arity t \<and> apply_guards (Guard t) (case_vname (\<lambda>n. if n = 1 then Some (Num 50) else input2state [] (1 + 1) (I n)) Map.empty))
-         {((1, 2), \<lparr>Label = (STR ''coin''), Arity = Suc 0, Guard = [gexp.Eq (V (I 1)) (L (Num 50))], Outputs = [L (Num 50)], Updates = []\<rparr>),
-          ((0, 1), \<lparr>Label = (STR ''select''), Arity = Suc 0, Guard = [gexp.Eq (V (I 1)) (L ((Str ''coke'')))], Outputs = [], Updates = []\<rparr>)} = {}"
-        by (simp add: Set.filter_def)
-      show ?thesis
-        by (simp add: step_def possible_steps_def ffilter_def set_filter)
-    qed
-    have step_vend_coke: "step
-           {|((2, 3), \<lparr>Label = (STR ''coin''), Arity = Suc 0, Guard = [gexp.Eq (V (I 1)) (L (Num 50))], Outputs = [L (Num 100)], Updates = []\<rparr>),
-             ((1, 2), \<lparr>Label = (STR ''coin''), Arity = Suc 0, Guard = [gexp.Eq (V (I 1)) (L (Num 50))], Outputs = [L (Num 50)], Updates = []\<rparr>),
-             ((0, 1), \<lparr>Label = (STR ''select''), Arity = Suc 0, Guard = [gexp.Eq (V (I 1)) (L ((Str ''coke'')))], Outputs = [], Updates = []\<rparr>)|}
-           3 Map.empty (STR ''vend'') [] = None"
-    proof-
-      have set_filter: "Set.filter (\<lambda>((origin, dest), t). origin = (3::nat) \<and> Label t = (STR ''vend'') \<and> Arity t = 0 \<and> apply_guards (Guard t) (case_vname Map.empty Map.empty))
-         {((2, 3), \<lparr>Label = (STR ''coin''), Arity = Suc 0, Guard = [gexp.Eq (V (I 1)) (L (Num 50))], Outputs = [L (Num 100)], Updates = []\<rparr>),
-          ((1, 2), \<lparr>Label = (STR ''coin''), Arity = Suc 0, Guard = [gexp.Eq (V (I 1)) (L (Num 50))], Outputs = [L (Num 50)], Updates = []\<rparr>),
-          ((0, 1), \<lparr>Label = (STR ''select''), Arity = Suc 0, Guard = [gexp.Eq (V (I 1)) (L ((Str ''coke'')))], Outputs = [], Updates = []\<rparr>)} = {}"
-        by (simp add: Set.filter_def)
-      show ?thesis
-        by (simp add: step_def possible_steps_def ffilter_def set_filter)
-    qed
-    have step_selectCoke_2: "step
-                  {|((3, 4), \<lparr>Label = (STR ''vend''), Arity = 0, Guard = [], Outputs = [L ((Str ''coke''))], Updates = []\<rparr>),
-                    ((2, 3), \<lparr>Label = (STR ''coin''), Arity = Suc 0, Guard = [gexp.Eq (V (I 1)) (L (Num 50))], Outputs = [L (Num 100)], Updates = []\<rparr>),
-                    ((1, 2), \<lparr>Label = (STR ''coin''), Arity = Suc 0, Guard = [gexp.Eq (V (I 1)) (L (Num 50))], Outputs = [L (Num 50)], Updates = []\<rparr>),
-                    ((0, 1), \<lparr>Label = (STR ''select''), Arity = Suc 0, Guard = [gexp.Eq (V (I 1)) (L ((Str ''coke'')))], Outputs = [], Updates = []\<rparr>)|}
-                  0 Map.empty (STR ''select'') [(Str ''coke'')] = Some (selectCoke, 1, [], <>)"
-    proof-
-      have set_filter: "Set.filter
-          (\<lambda>((origin, dest), t).
-              origin = 0 \<and>
-              Label t = (STR ''select'') \<and>
-              Suc 0 = Arity t \<and> apply_guards (Guard t) (case_vname (\<lambda>n. if n = 1 then Some ((Str ''coke'')) else input2state [] (1 + 1) (I n)) Map.empty))
-          {((3, 4), \<lparr>Label = (STR ''vend''), Arity = 0, Guard = [], Outputs = [L ((Str ''coke''))], Updates = []\<rparr>),
-           ((2, 3), \<lparr>Label = (STR ''coin''), Arity = Suc 0, Guard = [gexp.Eq (V (I 1)) (L (Num 50))], Outputs = [L (Num 100)], Updates = []\<rparr>),
-           ((1, 2), \<lparr>Label = (STR ''coin''), Arity = Suc 0, Guard = [gexp.Eq (V (I 1)) (L (Num 50))], Outputs = [L (Num 50)], Updates = []\<rparr>),
-           ((0, 1), \<lparr>Label = (STR ''select''), Arity = Suc 0, Guard = [gexp.Eq (V (I 1)) (L ((Str ''coke'')))], Outputs = [], Updates = []\<rparr>)} = {((0, 1), selectCoke)}"
-        apply (simp add: Set.filter_def)
-        apply safe
-        by (simp_all add: selectCoke_def)
-      show ?thesis
-        apply (simp add: step_def possible_steps_def ffilter_def set_filter)
-        by (simp add: set_filter selectCoke_def)
-    qed
-    have step_coin100: "step
-                  {|((3, 4), \<lparr>Label = (STR ''vend''), Arity = 0, Guard = [], Outputs = [L ((Str ''coke''))], Updates = []\<rparr>),
-                    ((2, 3), \<lparr>Label = (STR ''coin''), Arity = Suc 0, Guard = [gexp.Eq (V (I 1)) (L (Num 50))], Outputs = [L (Num 100)], Updates = []\<rparr>),
-                    ((1, 2), \<lparr>Label = (STR ''coin''), Arity = Suc 0, Guard = [gexp.Eq (V (I 1)) (L (Num 50))], Outputs = [L (Num 50)], Updates = []\<rparr>),
-                    ((0, 1), \<lparr>Label = (STR ''select''), Arity = Suc 0, Guard = [gexp.Eq (V (I 1)) (L ((Str ''coke'')))], Outputs = [], Updates = []\<rparr>)|}
-                  1 Map.empty (STR ''coin'') [Num 100] = None"
-    proof-
-      have applyGuards: "\<not> apply_guards [gexp.Eq (V (I 1)) (L (Num 50))] (case_vname (\<lambda>n. if n = 1 then Some (Num 100) else input2state [] (1 + 1) (I n)) Map.empty)"
-        by simp
-      have set_filter: "Set.filter
-         (\<lambda>((origin::nat, dest), t).
-             origin = 1 \<and>
-             Label t = (STR ''coin'') \<and>
-             Suc 0 = Arity t \<and> apply_guards (Guard t) (case_vname (\<lambda>n. if n = 1 then Some (Num 100) else input2state [] (1 + 1) (I n)) Map.empty))
-         {((3, 4), \<lparr>Label = (STR ''vend''), Arity = 0, Guard = [], Outputs = [L ((Str ''coke''))], Updates = []\<rparr>),
-          ((2, 3), \<lparr>Label = (STR ''coin''), Arity = Suc 0, Guard = [gexp.Eq (V (I 1)) (L (Num 50))], Outputs = [L (Num 100)], Updates = []\<rparr>),
-          ((1, 2), \<lparr>Label = (STR ''coin''), Arity = Suc 0, Guard = [gexp.Eq (V (I 1)) (L (Num 50))], Outputs = [L (Num 50)], Updates = []\<rparr>),
-          ((0, 1), \<lparr>Label = (STR ''select''), Arity = Suc 0, Guard = [gexp.Eq (V (I 1)) (L ((Str ''coke'')))], Outputs = [], Updates = []\<rparr>)} = {}"
-        apply (simp add: Set.filter_def)
-        apply clarify
-        using applyGuards
-        by (metis (no_types, lifting) select_convs(3))
-      show ?thesis
-        by (simp add: step_def possible_steps_def ffilter_def set_filter)
-    qed
-    have step_vend_coke_2: "step
-                  {|((1, 5), \<lparr>Label = (STR ''coin''), Arity = Suc 0, Guard = [gexp.Eq (V (I 1)) (L (Num 100))], Outputs = [L (Num 100)], Updates = []\<rparr>),
-                    ((3, 4), \<lparr>Label = (STR ''vend''), Arity = 0, Guard = [], Outputs = [L ((Str ''coke''))], Updates = []\<rparr>),
-                    ((2, 3), \<lparr>Label = (STR ''coin''), Arity = Suc 0, Guard = [gexp.Eq (V (I 1)) (L (Num 50))], Outputs = [L (Num 100)], Updates = []\<rparr>),
-                    ((1, 2), \<lparr>Label = (STR ''coin''), Arity = Suc 0, Guard = [gexp.Eq (V (I 1)) (L (Num 50))], Outputs = [L (Num 50)], Updates = []\<rparr>),
-                    ((0, 1), \<lparr>Label = (STR ''select''), Arity = Suc 0, Guard = [gexp.Eq (V (I 1)) (L ((Str ''coke'')))], Outputs = [], Updates = []\<rparr>)|}
-                  5 Map.empty (STR ''vend'') [] = None"
-    proof-
-      have set_filter: "Set.filter (\<lambda>((origin::nat, dest), t). origin = 5 \<and> Label t = (STR ''vend'') \<and> Arity t = 0 \<and> apply_guards (Guard t) (case_vname Map.empty Map.empty))
-         {((1, 5), \<lparr>Label = (STR ''coin''), Arity = Suc 0, Guard = [gexp.Eq (V (I 1)) (L (Num 100))], Outputs = [L (Num 100)], Updates = []\<rparr>),
-          ((3, 4), \<lparr>Label = (STR ''vend''), Arity = 0, Guard = [], Outputs = [L ((Str ''coke''))], Updates = []\<rparr>),
-          ((2, 3), \<lparr>Label = (STR ''coin''), Arity = Suc 0, Guard = [gexp.Eq (V (I 1)) (L (Num 50))], Outputs = [L (Num 100)], Updates = []\<rparr>),
-          ((1, 2), \<lparr>Label = (STR ''coin''), Arity = Suc 0, Guard = [gexp.Eq (V (I 1)) (L (Num 50))], Outputs = [L (Num 50)], Updates = []\<rparr>),
-          ((0, 1), \<lparr>Label = (STR ''select''), Arity = Suc 0, Guard = [gexp.Eq (V (I 1)) (L ((Str ''coke'')))], Outputs = [], Updates = []\<rparr>)} = {}"
-        by (simp add: Set.filter_def)
-      show ?thesis
-        by (simp add: step_def possible_steps_def ffilter_def set_filter)
-    qed
-    have step_select_pepsi: "step
-           {|((5, 6), \<lparr>Label = (STR ''vend''), Arity = 0, Guard = [], Outputs = [L ((Str ''coke''))], Updates = []\<rparr>),
-             ((1, 5), \<lparr>Label = (STR ''coin''), Arity = Suc 0, Guard = [gexp.Eq (V (I 1)) (L (Num 100))], Outputs = [L (Num 100)], Updates = []\<rparr>),
-             ((3, 4), \<lparr>Label = (STR ''vend''), Arity = 0, Guard = [], Outputs = [L ((Str ''coke''))], Updates = []\<rparr>),
-             ((2, 3), \<lparr>Label = (STR ''coin''), Arity = Suc 0, Guard = [gexp.Eq (V (I 1)) (L (Num 50))], Outputs = [L (Num 100)], Updates = []\<rparr>),
-             ((1, 2), \<lparr>Label = (STR ''coin''), Arity = Suc 0, Guard = [gexp.Eq (V (I 1)) (L (Num 50))], Outputs = [L (Num 50)], Updates = []\<rparr>),
-             ((0, 1), \<lparr>Label = (STR ''select''), Arity = Suc 0, Guard = [gexp.Eq (V (I 1)) (L ((Str ''coke'')))], Outputs = [], Updates = []\<rparr>)|}
-           0 Map.empty (STR ''select'') [(Str ''pepsi'')] = None"
-    proof-
-      have applyGuards: "\<not>apply_guards [gexp.Eq (V (I 1)) (L ((Str ''coke'')))] (case_vname (\<lambda>n. if n = 1 then Some ((Str ''pepsi'')) else input2state [] (1 + 1) (I n)) Map.empty)"
-        by (simp add: implode_coke implode_pepsi)
-      have set_filter: "Set.filter
-         (\<lambda>((origin::nat, dest::nat), t).
-             origin = 0 \<and>
-             Label t = (STR ''select'') \<and>
-             Suc 0 = Arity t \<and> apply_guards (Guard t) (case_vname (\<lambda>n. if n = 1 then Some ((Str ''pepsi'')) else input2state [] (1 + 1) (I n)) Map.empty))
-         {((5, 6), \<lparr>Label = (STR ''vend''), Arity = 0, Guard = [], Outputs = [L ((Str ''coke''))], Updates = []\<rparr>),
-          ((1, 5), \<lparr>Label = (STR ''coin''), Arity = Suc 0, Guard = [gexp.Eq (V (I 1)) (L (Num 100))], Outputs = [L (Num 100)], Updates = []\<rparr>),
-          ((3, 4), \<lparr>Label = (STR ''vend''), Arity = 0, Guard = [], Outputs = [L ((Str ''coke''))], Updates = []\<rparr>),
-          ((2, 3), \<lparr>Label = (STR ''coin''), Arity = Suc 0, Guard = [gexp.Eq (V (I 1)) (L (Num 50))], Outputs = [L (Num 100)], Updates = []\<rparr>),
-          ((1, 2), \<lparr>Label = (STR ''coin''), Arity = Suc 0, Guard = [gexp.Eq (V (I 1)) (L (Num 50))], Outputs = [L (Num 50)], Updates = []\<rparr>),
-          ((0, 1), \<lparr>Label = (STR ''select''), Arity = Suc 0, Guard = [gexp.Eq (V (I 1)) (L ((Str ''coke'')))], Outputs = [], Updates = []\<rparr>)} = {}"
-        apply (simp add: Set.filter_def)
-        apply clarify
-        by (metis (no_types, lifting) applyGuards select_convs(3))
-      show ?thesis
-        by (simp add: step_def possible_steps_def ffilter_def set_filter)
-    qed
-    have step_coin50_3:  "step
-           {|((0, 7), \<lparr>Label = (STR ''select''), Arity = Suc 0, Guard = [gexp.Eq (V (I 1)) (L ((Str ''pepsi'')))], Outputs = [], Updates = []\<rparr>),
-             ((5, 6), \<lparr>Label = (STR ''vend''), Arity = 0, Guard = [], Outputs = [L ((Str ''coke''))], Updates = []\<rparr>),
-             ((1, 5), \<lparr>Label = (STR ''coin''), Arity = Suc 0, Guard = [gexp.Eq (V (I 1)) (L (Num 100))], Outputs = [L (Num 100)], Updates = []\<rparr>),
-             ((3, 4), \<lparr>Label = (STR ''vend''), Arity = 0, Guard = [], Outputs = [L ((Str ''coke''))], Updates = []\<rparr>),
-             ((2, 3), \<lparr>Label = (STR ''coin''), Arity = Suc 0, Guard = [gexp.Eq (V (I 1)) (L (Num 50))], Outputs = [L (Num 100)], Updates = []\<rparr>),
-             ((1, 2), \<lparr>Label = (STR ''coin''), Arity = Suc 0, Guard = [gexp.Eq (V (I 1)) (L (Num 50))], Outputs = [L (Num 50)], Updates = []\<rparr>),
-             ((0, 1), \<lparr>Label = (STR ''select''), Arity = Suc 0, Guard = [gexp.Eq (V (I 1)) (L ((Str ''coke'')))], Outputs = [], Updates = []\<rparr>)|}
-           7 Map.empty (STR ''coin'') [Num 50] = None"
-    proof-
-      have set_filter: "Set.filter
-         (\<lambda>((origin::nat, dest::nat), t).
-             origin = 7 \<and>
-             Label t = (STR ''coin'') \<and>
-             Suc 0 = Arity t \<and> apply_guards (Guard t) (case_vname (\<lambda>n. if n = 1 then Some (Num 50) else input2state [] (1 + 1) (I n)) Map.empty))
-         {((0, 7), \<lparr>Label = (STR ''select''), Arity = Suc 0, Guard = [gexp.Eq (V (I 1)) (L ((Str ''pepsi'')))], Outputs = [], Updates = []\<rparr>),
-          ((5, 6), \<lparr>Label = (STR ''vend''), Arity = 0, Guard = [], Outputs = [L ((Str ''coke''))], Updates = []\<rparr>),
-          ((1, 5), \<lparr>Label = (STR ''coin''), Arity = Suc 0, Guard = [gexp.Eq (V (I 1)) (L (Num 100))], Outputs = [L (Num 100)], Updates = []\<rparr>),
-          ((3, 4), \<lparr>Label = (STR ''vend''), Arity = 0, Guard = [], Outputs = [L ((Str ''coke''))], Updates = []\<rparr>),
-          ((2, 3), \<lparr>Label = (STR ''coin''), Arity = Suc 0, Guard = [gexp.Eq (V (I 1)) (L (Num 50))], Outputs = [L (Num 100)], Updates = []\<rparr>),
-          ((1, 2), \<lparr>Label = (STR ''coin''), Arity = Suc 0, Guard = [gexp.Eq (V (I 1)) (L (Num 50))], Outputs = [L (Num 50)], Updates = []\<rparr>),
-          ((0, 1), \<lparr>Label = (STR ''select''), Arity = Suc 0, Guard = [gexp.Eq (V (I 1)) (L ((Str ''coke'')))], Outputs = [], Updates = []\<rparr>)} = {}"
-        by (simp add: Set.filter_def)
-    show ?thesis
-      by (simp add: step_def possible_steps_def ffilter_def set_filter)
-  qed
-  have step_coin50_4: "step
-           {|((7, 8), \<lparr>Label = (STR ''coin''), Arity = Suc 0, Guard = [gexp.Eq (V (I 1)) (L (Num 50))], Outputs = [L (Num 50)], Updates = []\<rparr>),
-             ((0, 7), \<lparr>Label = (STR ''select''), Arity = Suc 0, Guard = [gexp.Eq (V (I 1)) (L ((Str ''pepsi'')))], Outputs = [], Updates = []\<rparr>),
-             ((5, 6), \<lparr>Label = (STR ''vend''), Arity = 0, Guard = [], Outputs = [L ((Str ''coke''))], Updates = []\<rparr>),
-             ((1, 5), \<lparr>Label = (STR ''coin''), Arity = Suc 0, Guard = [gexp.Eq (V (I 1)) (L (Num 100))], Outputs = [L (Num 100)], Updates = []\<rparr>),
-             ((3, 4), \<lparr>Label = (STR ''vend''), Arity = 0, Guard = [], Outputs = [L ((Str ''coke''))], Updates = []\<rparr>),
-             ((2, 3), \<lparr>Label = (STR ''coin''), Arity = Suc 0, Guard = [gexp.Eq (V (I 1)) (L (Num 50))], Outputs = [L (Num 100)], Updates = []\<rparr>),
-             ((1, 2), \<lparr>Label = (STR ''coin''), Arity = Suc 0, Guard = [gexp.Eq (V (I 1)) (L (Num 50))], Outputs = [L (Num 50)], Updates = []\<rparr>),
-             ((0, 1), \<lparr>Label = (STR ''select''), Arity = Suc 0, Guard = [gexp.Eq (V (I 1)) (L ((Str ''coke'')))], Outputs = [], Updates = []\<rparr>)|}
-           8 Map.empty (STR ''coin'') [Num 50] = None"
-  proof-
-    have set_filter: "Set.filter
-         (\<lambda>((origin::nat, dest::nat), t).
-             origin = 8 \<and>
-             Label t = (STR ''coin'') \<and>
-             Suc 0 = Arity t \<and> apply_guards (Guard t) (case_vname (\<lambda>n. if n = 1 then Some (Num 50) else input2state [] (1 + 1) (I n)) Map.empty))
-         {((7, 8), \<lparr>Label = (STR ''coin''), Arity = Suc 0, Guard = [gexp.Eq (V (I 1)) (L (Num 50))], Outputs = [L (Num 50)], Updates = []\<rparr>),
-          ((0, 7), \<lparr>Label = (STR ''select''), Arity = Suc 0, Guard = [gexp.Eq (V (I 1)) (L ((Str ''pepsi'')))], Outputs = [], Updates = []\<rparr>),
-          ((5, 6), \<lparr>Label = (STR ''vend''), Arity = 0, Guard = [], Outputs = [L ((Str ''coke''))], Updates = []\<rparr>),
-          ((1, 5), \<lparr>Label = (STR ''coin''), Arity = Suc 0, Guard = [gexp.Eq (V (I 1)) (L (Num 100))], Outputs = [L (Num 100)], Updates = []\<rparr>),
-          ((3, 4), \<lparr>Label = (STR ''vend''), Arity = 0, Guard = [], Outputs = [L ((Str ''coke''))], Updates = []\<rparr>),
-          ((2, 3), \<lparr>Label = (STR ''coin''), Arity = Suc 0, Guard = [gexp.Eq (V (I 1)) (L (Num 50))], Outputs = [L (Num 100)], Updates = []\<rparr>),
-          ((1, 2), \<lparr>Label = (STR ''coin''), Arity = Suc 0, Guard = [gexp.Eq (V (I 1)) (L (Num 50))], Outputs = [L (Num 50)], Updates = []\<rparr>),
-          ((0, 1), \<lparr>Label = (STR ''select''), Arity = Suc 0, Guard = [gexp.Eq (V (I 1)) (L ((Str ''coke'')))], Outputs = [], Updates = []\<rparr>)} = {}"
-      by (simp add: Set.filter_def)
-    show ?thesis
-      by (simp add: step_def possible_steps_def ffilter_def set_filter)
-  qed
-  have step_vend_pepsi: "step
-           {|((8, 9), \<lparr>Label = (STR ''coin''), Arity = Suc 0, Guard = [gexp.Eq (V (I 1)) (L (Num 50))], Outputs = [L (Num 100)], Updates = []\<rparr>),
-             ((7, 8), \<lparr>Label = (STR ''coin''), Arity = Suc 0, Guard = [gexp.Eq (V (I 1)) (L (Num 50))], Outputs = [L (Num 50)], Updates = []\<rparr>),
-             ((0, 7), \<lparr>Label = (STR ''select''), Arity = Suc 0, Guard = [gexp.Eq (V (I 1)) (L ((Str ''pepsi'')))], Outputs = [], Updates = []\<rparr>),
-             ((5, 6), \<lparr>Label = (STR ''vend''), Arity = 0, Guard = [], Outputs = [L ((Str ''coke''))], Updates = []\<rparr>),
-             ((1, 5), \<lparr>Label = (STR ''coin''), Arity = Suc 0, Guard = [gexp.Eq (V (I 1)) (L (Num 100))], Outputs = [L (Num 100)], Updates = []\<rparr>),
-             ((3, 4), \<lparr>Label = (STR ''vend''), Arity = 0, Guard = [], Outputs = [L ((Str ''coke''))], Updates = []\<rparr>),
-             ((2, 3), \<lparr>Label = (STR ''coin''), Arity = Suc 0, Guard = [gexp.Eq (V (I 1)) (L (Num 50))], Outputs = [L (Num 100)], Updates = []\<rparr>),
-             ((1, 2), \<lparr>Label = (STR ''coin''), Arity = Suc 0, Guard = [gexp.Eq (V (I 1)) (L (Num 50))], Outputs = [L (Num 50)], Updates = []\<rparr>),
-             ((0, 1), \<lparr>Label = (STR ''select''), Arity = Suc 0, Guard = [gexp.Eq (V (I 1)) (L ((Str ''coke'')))], Outputs = [], Updates = []\<rparr>)|}
-           9 Map.empty (STR ''vend'') [] = None"
-  proof-
-    have set_filter: "Set.filter (\<lambda>((origin::nat, dest::nat), t). origin = 9 \<and> Label t = (STR ''vend'') \<and> Arity t = 0 \<and> apply_guards (Guard t) (case_vname Map.empty Map.empty))
-         {((8, 9), \<lparr>Label = (STR ''coin''), Arity = Suc 0, Guard = [gexp.Eq (V (I 1)) (L (Num 50))], Outputs = [L (Num 100)], Updates = []\<rparr>),
-         ((7, 8), \<lparr>Label = (STR ''coin''), Arity = Suc 0, Guard = [gexp.Eq (V (I 1)) (L (Num 50))], Outputs = [L (Num 50)], Updates = []\<rparr>),
-         ((0, 7), \<lparr>Label = (STR ''select''), Arity = Suc 0, Guard = [gexp.Eq (V (I 1)) (L ((Str ''pepsi'')))], Outputs = [], Updates = []\<rparr>),
-         ((5, 6), \<lparr>Label = (STR ''vend''), Arity = 0, Guard = [], Outputs = [L ((Str ''coke''))], Updates = []\<rparr>),
-         ((1, 5), \<lparr>Label = (STR ''coin''), Arity = Suc 0, Guard = [gexp.Eq (V (I 1)) (L (Num 100))], Outputs = [L (Num 100)], Updates = []\<rparr>),
-         ((3, 4), \<lparr>Label = (STR ''vend''), Arity = 0, Guard = [], Outputs = [L ((Str ''coke''))], Updates = []\<rparr>),
-         ((2, 3), \<lparr>Label = (STR ''coin''), Arity = Suc 0, Guard = [gexp.Eq (V (I 1)) (L (Num 50))], Outputs = [L (Num 100)], Updates = []\<rparr>),
-         ((1, 2), \<lparr>Label = (STR ''coin''), Arity = Suc 0, Guard = [gexp.Eq (V (I 1)) (L (Num 50))], Outputs = [L (Num 50)], Updates = []\<rparr>),
-         ((0, 1), \<lparr>Label = (STR ''select''), Arity = Suc 0, Guard = [gexp.Eq (V (I 1)) (L ((Str ''coke'')))], Outputs = [], Updates = []\<rparr>)} = {}"
-      by (simp add: Set.filter_def)
-    show ?thesis
-      by (simp add: step_def possible_steps_def ffilter_def set_filter)
-  qed
-  have select_coke: " \<lparr>Label = (STR ''select''), Arity = Suc 0, Guard = [gexp.Eq (V (I 1)) (L ((Str ''coke'')))], Outputs = [], Updates = []\<rparr> = selectCoke"
-    by (simp add: selectCoke_def)
-  have coin50_50: "\<lparr>Label = (STR ''coin''), Arity = Suc 0, Guard = [gexp.Eq (V (I 1)) (L (Num 50))], Outputs = [L (Num 50)], Updates = []\<rparr> = coin50_50"
-    by (simp add: coin50_50_def)
-  have coin100_100: " \<lparr>Label = (STR ''coin''), Arity = Suc 0, Guard = [gexp.Eq (V (I 1)) (L (Num 100))], Outputs = [L (Num 100)], Updates = []\<rparr> = coin100_100"
-    by (simp add: coin100_100_def)
-  have coin50_100: "\<lparr>Label = (STR ''coin''), Arity = Suc 0, Guard = [gexp.Eq (V (I 1)) (L (Num 50))], Outputs = [L (Num 100)], Updates = []\<rparr> = coin50_100"
-    by (simp add: coin50_100_def)
-  have selectPepsi: "\<lparr>Label = (STR ''select''), Arity = Suc 0, Guard = [gexp.Eq (V (I 1)) (L ((Str ''pepsi'')))], Outputs = [], Updates = []\<rparr> = selectPepsi"
-    by (simp add: selectPepsi_def)
-  have vendCoke: "\<lparr>Label = (STR ''vend''), Arity = 0, Guard = [], Outputs = [L ((Str ''coke''))], Updates = []\<rparr> = vend_coke"
-    by (simp add: vend_coke_def)
-  have vendPepsi: "\<lparr>Label = (STR ''vend''), Arity = 0, Guard = [], Outputs = [L ((Str ''pepsi''))], Updates = []\<rparr> = vend_pepsi"
-    by (simp add: vend_pepsi_def)
-  have sorted_list_of_fset: "sorted_list_of_fset
-         {|((9::nat, 10::nat), vend_pepsi), ((8, 9), coin50_100), ((7, 8), coin50_50), ((0, 7), selectPepsi), ((5, 6), vend_coke),
-           ((1, 5), coin100_100), ((3, 4), vend_coke), ((2, 3), coin50_100), ((1, 2), coin50_50), ((0, 1), selectCoke)|} = [((0, 1), selectCoke), ((0, 7), selectPepsi), ((1, 2), coin50_50), ((1, 5), coin100_100), ((2, 3), coin50_100), ((3, 4), vend_coke),
-     ((5, 6), vend_coke), ((7, 8), coin50_50), ((8, 9), coin50_100), ((9, 10), vend_pepsi)]"
-    by (simp add: sorted_list_of_fset_def )
-  show ?thesis
-    apply (simp add: make_pta_def traces_def)
-    apply (simp add: step_coin50 step_coin50_2 step_vend_coke
-                      step_selectCoke_2 step_coin100 step_vend_coke_2
-                      step_select_pepsi step_coin50_3 step_coin50_4 step_vend_pepsi)
-    apply (simp add: select_coke coin50_50 coin100_100 coin50_100 selectPepsi vendCoke vendPepsi)
-    apply (simp add: toiEFSM_def toiEFSM_aux_def)
-    apply (simp add: sorted_list_of_fset pta_def)
-    by auto
-qed
 
 definition filtered_pairs :: "(nat \<times> nat) set" where
   "filtered_pairs = {(9, 10), (8, 10), (8, 9), (7, 10), (7, 9), (7, 8), (6, 10), (6, 9), (6, 8), (6, 7), (5, 10), (5, 9), (5, 8), (5, 7), (5, 6), (4, 10),
@@ -375,185 +99,177 @@ proof-
     apply (simp add: outgoing_transitions_def pta_def fimage_def)
     apply (simp add: naive_score_empty set_equiv)
     apply (simp add: naive_score_def fprod_def)
-    by (simp add: transitions Abs_fset_inverse)
+    by (simp add: Abs_fset_inverse)
   show ?thesis
     by (simp add: scores sorted_list_of_fset_def)
 qed
 
 lemmas possible_steps_fst = possible_steps_def ffilter_def fimage_def fset_both_sides Abs_fset_inverse
 
-lemma step_pta_coin50_7: "step (tm pta) 7 r (STR ''coin'') [Num 50] = Some (coin50_50, 8, [Some (Num 50)], r)"
+lemma step_pta_coin50_7: "step (tm pta) 7 r (STR ''coin'') [Num 50] = Some (coin 50 50, 8, [Some (Num 50)], r)"
 proof-
-  have possible_steps: "possible_steps (tm pta) 7 r (STR ''coin'') [Num 50] = {|(8, coin50_50)|}"
+  have possible_steps: "possible_steps (tm pta) 7 r (STR ''coin'') [Num 50] = {|(8, coin 50 50)|}"
     apply (simp add: possible_steps_fst)
     apply (simp add: Set.filter_def tm_def pta_def)
     apply safe
-                     apply (simp_all add: transitions)
+                     apply simp_all
     by force
   show ?thesis
-    apply (simp add: step_def possible_steps)
-    by (simp add: coin50_50_def)
+    by (simp add: step_def possible_steps)
 qed
 
-lemma step_pta_coin50_1: "step (tm pta) 1 r (STR ''coin'') [Num 50] = Some (coin50_50, 2, [Some (Num 50)], r)"
+lemma step_pta_coin50_1: "step (tm pta) 1 r (STR ''coin'') [Num 50] = Some (coin 50 50, 2, [Some (Num 50)], r)"
 proof-
-  have possible_steps: "possible_steps (tm pta) 1 r (STR ''coin'') [Num 50] = {|(2, coin50_50)|}"
+  have possible_steps: "possible_steps (tm pta) 1 r (STR ''coin'') [Num 50] = {|(2, coin 50 50)|}"
     apply (simp add: possible_steps_fst)
     apply (simp add: Set.filter_def tm_def pta_def)
     apply safe
-                     apply (simp_all add: transitions)
+                     apply simp_all
     by force
   show ?thesis
-    apply (simp add: step_def possible_steps)
-    by (simp add: coin50_50_def)
+    by (simp add: step_def possible_steps)
 qed
 
-lemma step_pta_vend_5: "step (tm pta) 5 r (STR ''vend'') [] = Some (vend_coke, 6, [Some ((Str ''coke''))], r)"
+lemma step_pta_vend_5: "step (tm pta) 5 r (STR ''vend'') [] = Some ((vend coke), 6, [Some ((Str ''coke''))], r)"
 proof-
-  have possible_steps: "possible_steps (tm pta) 5 r (STR ''vend'') [] = {|(6, vend_coke)|}"
+  have possible_steps: "possible_steps (tm pta) 5 r (STR ''vend'') [] = {|(6, (vend coke))|}"
     apply (simp add: possible_steps_fst)
     apply (simp add: Set.filter_def tm_def pta_def)
     apply safe
-                     apply (simp_all add: transitions)
+                     apply simp_all
     by force
   show ?thesis
     apply (simp add: step_def possible_steps)
-    by (simp add: transitions)
+    by (simp add: implode_coke)
 qed
 
-lemma step_pta_coin100_1: "step (tm pta) 1 r (STR ''coin'') [Num 100] = Some (coin100_100, 5, [Some (Num 100)], r)"
+lemma step_pta_coin100_1: "step (tm pta) 1 r (STR ''coin'') [Num 100] = Some (coin 100 100, 5, [Some (Num 100)], r)"
 proof-
-  have possible_steps: "possible_steps (tm pta) 1 r (STR ''coin'') [Num 100] = {|(5, coin100_100)|}"
+  have possible_steps: "possible_steps (tm pta) 1 r (STR ''coin'') [Num 100] = {|(5, coin 100 100)|}"
     apply (simp add: possible_steps_fst)
     apply (simp add: Set.filter_def tm_def pta_def)
     apply safe
-                     apply (simp_all add: transitions)
+                     apply simp_all
     by force
   show ?thesis
-    apply (simp add: step_def possible_steps)
-    by (simp add: coin100_100_def)
+    by (simp add: step_def possible_steps)
 qed
 
-lemma step_pta_coin50_2: "step (tm pta) 2 r (STR ''coin'') [Num 50] = Some (coin50_100, 3, [Some (Num 100)], r)"
+lemma step_pta_coin50_2: "step (tm pta) 2 r (STR ''coin'') [Num 50] = Some (coin 50 100, 3, [Some (Num 100)], r)"
 proof-
-  have possible_steps: "possible_steps (tm pta) 2 r (STR ''coin'') [Num 50] = {|(3, coin50_100)|}"
+  have possible_steps: "possible_steps (tm pta) 2 r (STR ''coin'') [Num 50] = {|(3, coin 50 100)|}"
     apply (simp add: possible_steps_fst)
     apply (simp add: Set.filter_def tm_def pta_def)
     apply safe
-                     apply (simp_all add: transitions)
+                     apply (simp_all add:)
     by force
   show ?thesis
-    apply (simp add: step_def possible_steps)
-    by (simp add: coin50_100_def)
+    by (simp add: step_def possible_steps)
 qed
 
-lemma step_pta_coin50_8: "step (tm pta) 8 r (STR ''coin'') [Num 50] = Some (coin50_100, 9, [Some (Num 100)], r)"
+lemma step_pta_coin50_8: "step (tm pta) 8 r (STR ''coin'') [Num 50] = Some (coin 50 100, 9, [Some (Num 100)], r)"
 proof-
-  have possible_steps: "possible_steps (tm pta) 8 r (STR ''coin'') [Num 50] = {|(9, coin50_100)|}"
+  have possible_steps: "possible_steps (tm pta) 8 r (STR ''coin'') [Num 50] = {|(9, coin 50 100)|}"
     apply (simp add: possible_steps_fst)
     apply (simp add: Set.filter_def tm_def pta_def)
     apply safe
-                     apply (simp_all add: transitions)
+                     apply simp_all
     by force
   show ?thesis
-    apply (simp add: step_def possible_steps)
-    by (simp add: coin50_100_def)
+    by (simp add: step_def possible_steps)
 qed
 
-lemma step_pta_vend_3: "step (tm pta) 3 r (STR ''vend'') [] = Some (vend_coke, 4, [Some ((Str ''coke''))], r)"
+lemma step_pta_vend_3: "step (tm pta) 3 r (STR ''vend'') [] = Some ((vend coke), 4, [Some ((Str ''coke''))], r)"
 proof-
-  have possible_steps: "possible_steps (tm pta) 3 r (STR ''vend'') [] = {|(4, vend_coke)|}"
+  have possible_steps: "possible_steps (tm pta) 3 r (STR ''vend'') [] = {|(4, (vend coke))|}"
     apply (simp add: possible_steps_fst)
     apply (simp add: Set.filter_def tm_def pta_def)
     apply safe
-                     apply (simp_all add: transitions)
+                     apply simp_all
     by force
   show ?thesis
-    apply (simp add: step_def possible_steps)
-    by (simp add: vend_coke_def)
+    by (simp add: step_def possible_steps implode_coke)
 qed
 
-lemma step_pta_vend_9: "step (tm pta) 9 r (STR ''vend'') [] = Some (vend_pepsi, 10, [Some ((Str ''pepsi''))], r)"
+lemma step_pta_vend_9: "step (tm pta) 9 r (STR ''vend'') [] = Some ((vend pepsi), 10, [Some ((Str ''pepsi''))], r)"
 proof-
-  have possible_steps: "possible_steps (tm pta) 9 r (STR ''vend'') [] = {|(10, vend_pepsi)|}"
+  have possible_steps: "possible_steps (tm pta) 9 r (STR ''vend'') [] = {|(10, (vend pepsi))|}"
     apply (simp add: possible_steps_fst)
     apply (simp add: Set.filter_def tm_def pta_def)
     apply safe
-                     apply (simp_all add: transitions)
+                     apply simp_all
     by force
   show ?thesis
-    apply (simp add: step_def possible_steps)
-    by (simp add: vend_pepsi_def)
+    by (simp add: step_def possible_steps implode_pepsi)
 qed
 
 definition merged_1_8 :: iEFSM where
   "merged_1_8 = {|
-(0, (0, 1), selectCoke),
-(1, (0, 7), selectPepsi),
-(2, (1, 2), coin50_50),
-(3, (1, 5), coin100_100),
-(4, (2, 3), coin50_100),
-(5, (3, 4), vend_coke),
-(6, (5, 6), vend_coke),
-(7, (7, 1), coin50_50),
-(8, (1, 9), coin50_100),
-(9, (9, 10), vend_pepsi)
+(0, (0, 1), select coke),
+(1, (0, 7), select pepsi),
+(2, (1, 2), coin 50 50),
+(3, (1, 5), coin 100 100),
+(4, (2, 3), coin 50 100),
+(5, (3, 4), (vend coke)),
+(6, (5, 6), (vend coke)),
+(7, (7, 1), coin 50 50),
+(8, (1, 9), coin 50 100),
+(9, (9, 10), (vend pepsi))
 |}"
 
 definition merged_2_9 :: iEFSM where
-  "merged_2_9 = {|(0, (0, 1), selectCoke), (1, (0, 7), selectPepsi), (2, (1, 2), coin50_50), (3, (1, 5), coin100_100), (4, (2, 3), coin50_100),
-      (5, (3, 4), vend_coke), (6, (5, 6), vend_coke), (7, (7, 1), coin50_50), (8, (1, 2), coin50_100), (9, (2, 10), vend_pepsi)|}"
+  "merged_2_9 = {|(0, (0, 1), select coke), (1, (0, 7), select pepsi), (2, (1, 2), coin 50 50), (3, (1, 5), coin 100 100), (4, (2, 3), coin 50 100),
+      (5, (3, 4), (vend coke)), (6, (5, 6), (vend coke)), (7, (7, 1), coin 50 50), (8, (1, 2), coin 50 100), (9, (2, 10), (vend pepsi))|}"
 
 lemma merge_states_2_9: "merge_states 2 9 merged_1_8 = merged_2_9 \<and> merge_states 9 2 merged_1_8 = merged_2_9"
   by (simp add: merge_states_def merge_states_aux_def merged_1_8_def merged_2_9_def)
 
-lemma no_subsumption_coin50_100_coin50_50: "\<not> subsumes c coin50_100 coin50_50"
-  by (simp add: subsumes_def transitions)
+lemma no_subsumption_coin_50_100_coin_50_50: "\<not> subsumes c (coin 50 100) (coin 50 50)"
+  by (simp add: subsumes_def)
 
-lemma no_subsumption_coin50_50_coin50_100: "\<not> subsumes c coin50_50 coin50_100"
-  by (simp add: subsumes_def transitions)
+lemma no_subsumption_coin_50_50_coin_50_100: "\<not> subsumes c (coin 50 50) (coin 50 100)"
+  by (simp add: subsumes_def)
 
-lemma no_subsumption_vend_coke_vend_pepsi: "\<not> subsumes c vend_coke vend_pepsi"
-  by (simp add: subsumes_def transitions Str_coke implode_pepsi)
+lemma no_subsumption_vend_coke_vend_pepsi: "\<not> subsumes c (vend coke) (vend pepsi)"
+  by (simp add: subsumes_def Str_coke implode_pepsi)
 
-lemma vend_pepsi_not_subsumes_vend_coke: "\<not> subsumes c vend_pepsi vend_coke"
-  by (simp add: subsumes_def transitions Str_coke implode_pepsi)
+lemma vend_pepsi_not_subsumes_vend_coke: "\<not> subsumes c (vend pepsi) (vend coke)"
+  by (simp add: subsumes_def Str_coke implode_pepsi)
 
-lemma step_pta_selectCoke: "step (tm pta) 0 Map.empty (STR ''select'') [(Str ''coke'')] = Some (selectCoke, 1, [], <>)"
+lemma step_pta_select_coke: "step (tm pta) 0 Map.empty (STR ''select'') [(Str ''coke'')] = Some (select coke, 1, [], <>)"
 proof-
-  have possible_steps: "possible_steps (tm pta) 0 Map.empty (STR ''select'') [(Str ''coke'')] = {|(1, selectCoke)|}"
+  have possible_steps: "possible_steps (tm pta) 0 Map.empty (STR ''select'') [(Str ''coke'')] = {|(1, select coke)|}"
     apply (simp add: possible_steps_def ffilter_def fimage_def fset_both_sides Abs_fset_inverse)
     apply (simp add: tm_def pta_def Set.filter_def)
     apply safe
-                      apply (simp_all add: transitions implode_coke implode_pepsi)
+                      apply (simp_all add:  implode_coke implode_pepsi)
     using Str_coke by force
   show ?thesis
-    apply (simp add: step_def possible_steps)
-    by (simp add: selectCoke_def)
+    by (simp add: step_def possible_steps)
 qed
 
 definition merged_1_7 :: iEFSM where
-  "merged_1_7 = {|(0, (0, 1), selectCoke), (2, (1, 2), coin50_50), (4, (2, 3), coin50_100),  (5, (3, 4), vend_coke), 
-                                                                   (3, (1, 5), coin100_100), (6, (5, 6), vend_coke),
-                 (1, (0, 1), selectPepsi), (7, (1, 8), coin50_50), (8, (8, 9), coin50_100),  (9, (9, 10), vend_pepsi)|}"
+  "merged_1_7 = {|(0, (0, 1), select coke), (2, (1, 2), coin 50 50), (4, (2, 3), coin 50 100),  (5, (3, 4), (vend coke)), 
+                                                                   (3, (1, 5), coin 100 100), (6, (5, 6), (vend coke)),
+                 (1, (0, 1), select pepsi), (7, (1, 8), coin 50 50), (8, (8, 9), coin 50 100),  (9, (9, 10), (vend pepsi))|}"
 
 lemma merge_states_1_7: "merge_states 1 7 pta = merged_1_7"
   by (simp add: merge_states_def pta_def merge_states_aux_def merged_1_7_def)
 
 definition merged_2_8 :: iEFSM where
-  "merged_2_8 = {|(0, (0, 1), selectCoke),  (2, (1, 2), coin50_50),  (4, (2, 3), coin50_100),  (5, (3, 4), vend_coke),
-                                                                      (3, (1, 5), coin100_100), (6, (5, 6), vend_coke),
-                   (1, (0, 1), selectPepsi), (7, (1, 2), coin50_50),  (8, (2, 9), coin50_100),  (9, (9, 10), vend_pepsi)|}"
+  "merged_2_8 = {|(0, (0, 1), select coke),  (2, (1, 2), coin 50 50),  (4, (2, 3), coin 50 100),  (5, (3, 4), (vend coke)),
+                                                                      (3, (1, 5), coin 100 100), (6, (5, 6), (vend coke)),
+                   (1, (0, 1), select pepsi), (7, (1, 2), coin 50 50),  (8, (2, 9), coin 50 100),  (9, (9, 10), (vend pepsi))|}"
 
 lemma merge_states_2_8: "merge_states 2 8 merged_1_7 = merged_2_8 \<and> merge_states 8 2 merged_1_7 = merged_2_8"
   by (simp add: merge_states_def merge_states_aux_def merged_1_7_def merged_2_8_def)
 
-lemma no_choice_coin50_50_coin100_100: "\<not>choice coin50_50 coin100_100"
-  by (simp add: choice_def transitions)
+lemma no_choice_coin_50_50_coin_100_100: "\<not>choice (coin 50 50) (coin 100 100)"
+  by (simp add: choice_def)
 
 definition merge_2_8_no_nondet :: iEFSM where
-  "merge_2_8_no_nondet = {|(0, (0, 1), selectCoke), (2, (1, 2), coin50_50), (4, (2, 3), coin50_100), (5, (3, 4), vend_coke), (3, (1, 5), coin100_100),
-      (6, (5, 6), vend_coke), (1, (0, 1), selectPepsi), (7, (1, 2), coin50_50), (8, (2, 9), coin50_100), (9, (9, 10), vend_pepsi)|}"
+  "merge_2_8_no_nondet = {|(0, (0, 1), select coke), (2, (1, 2), coin 50 50), (4, (2, 3), coin 50 100), (5, (3, 4), (vend coke)), (3, (1, 5), coin 100 100),
+      (6, (5, 6), (vend coke)), (1, (0, 1), select pepsi), (7, (1, 2), coin 50 50), (8, (2, 9), coin 50 100), (9, (9, 10), (vend pepsi))|}"
 
 definition selectGeneral :: transition where
   "selectGeneral = \<lparr>Label = (STR ''select''), Arity = 1, Guard = [], Outputs = [], Updates = [(R 1, V (I 1))]\<rparr>"
@@ -562,99 +278,41 @@ definition vend_general :: transition where
   "vend_general = \<lparr>Label = (STR ''vend''), Arity = 0, Guard = [], Outputs = [V (R 1)], Updates = []\<rparr>"
 
 definition merged_4_10 :: iEFSM where
-  "merged_4_10 = {|(0, (0, 1), selectCoke), (7, (1, 2), coin50_50), (8, (2, 3), coin50_100), (5, (3, 4), vend_coke) ,
-                   (1, (0, 1), selectPepsi),                                     (9, (3, 4), vend_pepsi), 
-                                            (3, (1, 5), coin100_100), (6, (5, 6), vend_coke)|}"
+  "merged_4_10 = {|(0, (0, 1), select coke), (7, (1, 2), coin 50 50), (8, (2, 3), coin 50 100), (5, (3, 4), (vend coke)) ,
+                   (1, (0, 1), select pepsi),                                     (9, (3, 4), (vend pepsi)), 
+                                            (3, (1, 5), coin 100 100), (6, (5, 6), (vend coke))|}"
 
 definition merged_vends :: iEFSM where
-  "merged_vends = {|(0, (0, 1), selectGeneral), (2, (1, 2), coin50_50), (4, (2, 3), coin50_100), (5, (3, 4), vend_general) ,
-                                            (3, (1, 5), coin100_100), (6, (5, 6), vend_general)|}"
+  "merged_vends = {|(0, (0, 1), selectGeneral), (2, (1, 2), coin 50 50), (4, (2, 3), coin 50 100), (5, (3, 4), vend_general) ,
+                                            (3, (1, 5), coin 100 100), (6, (5, 6), vend_general)|}"
 
 definition coinGeneral :: transition where
   "coinGeneral = \<lparr>Label = (STR ''coin''), Arity = 1, Guard = [], Outputs = [Plus (V (I 1)) (V (R 2))], Updates = [(R 2, Plus (V (I 1)) (V (R 2)))]\<rparr>"
-
-lemma no_choice_coin100_100_coin50_50: "\<not>choice coin100_100 coin50_50"
-  by (simp add: choice_def transitions)
-
-lemma no_choice_coin100_100_coin50_100: "\<not>choice coin100_100 coin50_100"
-  by (simp add: choice_def transitions)
-
-lemma no_choice_selectCoke_selectPepsi: "\<not>choice selectCoke selectPepsi"
-  by (simp add: choice_def transitions Str_coke Str_pepsi)
-
-lemma choice_coin50_100_coin50_50: "choice coin50_100 coin50_50"
-  apply (simp add: choice_def transitions)
-  by auto
-
-lemma choice_coin50_50_coin50_50: "choice coin50_50 coin50_50"
-  apply (simp add: choice_def transitions)
-  by auto
-
-lemma choice_coin50_100_coin50_100: "choice coin50_100 coin50_100"
-  apply (simp add: choice_def transitions)
-  by auto
-
-lemma choice_vend_coke_vend_pepsi: "choice vend_coke vend_pepsi"
-  by (simp add: choice_def transitions)
-
-lemma no_coice_vend_general_coin100_100:  "\<not>choice vend_general coin100_100"
-  by (simp add: choice_def transitions vend_general_def)
-
-lemma no_choice_coinGeneral_vend_general: "\<not>choice coinGeneral vend_general"
-  by (simp add: choice_def coinGeneral_def vend_general_def)
-
-lemma choice_coinGeneral_coin100_100: "choice coinGeneral coin100_100"
-  apply (simp add: transitions coinGeneral_def choice_def)
-  by auto
-
-lemma no_coice_coin100_100_vend_general: "\<not>choice coin100_100 vend_general"
-  by (simp add: choice_def transitions vend_general_def)
-
-lemma choice_coin100_100_coinGeneral: "choice coin100_100 coinGeneral"
-  apply (simp add: transitions coinGeneral_def choice_def)
-  by auto
-
-lemma choice_vend_general_vend_general: "choice vend_general vend_general"
-  by (simp add: choice_def vend_general_def)
-
-lemmas choices = choice_vend_general_vend_general choice_coin100_100_coinGeneral  no_coice_coin100_100_vend_general choice_coinGeneral_coin100_100 no_choice_coinGeneral_vend_general no_coice_vend_general_coin100_100 choice_vend_coke_vend_pepsi choice_coin50_100_coin50_100 choice_coin50_50_coin50_50 choice_coin50_100_coin50_50 no_choice_selectCoke_selectPepsi no_choice_coin100_100_coin50_100 no_choice_coin100_100_coin50_50 no_choice_coin50_50_coin100_100 choice_symmetry
-
-lemma coin50_50_lt_coin50_100: "coin50_50 < coin50_100"
-  by (simp add: transitions less_transition_ext_def less_aexp_def)
-
-lemma vend_coke_lt_vend_pepsi: "vend_coke < vend_pepsi"
-  apply (simp add: transitions less_transition_ext_def less_aexp_def Str_coke Str_pepsi)
-  by (simp add: String.less_literal_def explode_coke explode_pepsi)
-
-lemmas orders = vend_coke_lt_vend_pepsi coin50_50_lt_coin50_100
 
 lemma merge_states_1_8: "merge_states 1 8 pta = merged_1_8"
   apply (simp add: merge_states_def merge_states_aux_def pta_def merged_1_8_def)
   by auto
 
 lemma nondeterministic_pairs_merged_1_8: "nondeterministic_pairs merged_1_8 = {|
-    (1, (9, 2), (coin50_100, 8), coin50_50, 2),
-    (1, (2, 9), (coin50_50, 2), coin50_100, 8)
+    (1, (9, 2), (coin 50 100, 8), coin 50 50, 2),
+    (1, (2, 9), (coin 50 50, 2), coin 50 100, 8)
   |}"
 proof-
-  have minus_1: "{|(1, selectCoke, 0), (7, selectPepsi, 1)|} |-| {|(7, selectPepsi, 1)|} = {|(1, selectCoke, 0)|}"
-    apply (simp add: transitions Str_coke Str_pepsi)
+  have minus_1: "{|(1, select coke, 0), (7, select pepsi, 1)|} |-| {|(7, select pepsi, 1)|} = {|(1, select coke, 0)|}"
     by auto
-  have minus_2: "{|(2, coin50_50, 2), (5, coin100_100, 3), (9, coin50_100, 8)|} |-| {|(5, coin100_100, 3)|} = {|(2, coin50_50, 2), (9, coin50_100, 8)|}"
-    apply (simp add: transitions)
+  have minus_2: "{|(2, coin 50 50, 2), (5, coin 100 100, 3), (9, coin 50 100, 8)|} |-| {|(5, coin 100 100, 3)|} = {|(2, coin 50 50, 2), (9, coin 50 100, 8)|}"
     by auto
-  have minus_3: "{|(2, coin50_50, 2), (5, coin100_100, 3), (9, coin50_100, 8)|} |-| {|(9, coin50_100, 8)|} = {|(2, coin50_50, 2), (5, coin100_100, 3)|}"
-    apply (simp add: transitions)
+  have minus_3: "{|(2, coin 50 50, 2), (5, coin 100 100, 3), (9, coin 50 100, 8)|} |-| {|(9, coin 50 100, 8)|} = {|(2, coin 50 50, 2), (5, coin 100 100, 3)|}"
     by auto
-  have state_nondeterminsm_0: "state_nondeterminism 0 {|(1, selectCoke, 0), (7, selectPepsi, 1)|} = {|(0, (7, 1), (selectPepsi, 1), selectCoke, 0), (0, (1, 7), (selectCoke, 0), selectPepsi, 1) |}"
+  have state_nondeterminsm_0: "state_nondeterminism 0 {|(1, select coke, 0), (7, select pepsi, 1)|} = {|(0, (7, 1), (select pepsi, 1), select coke, 0), (0, (1, 7), (select coke, 0), select pepsi, 1) |}"
     by (simp add: state_nondeterminism_def minus_1)
-  have state_nondeterminism_1: "state_nondeterminism 1 {|(2, coin50_50, 2), (5, coin100_100, 3), (9, coin50_100, 8)|} = {|
-   (1, (9, 5), (coin50_100, 8), coin100_100, 3),
-   (1, (9, 2), (coin50_100, 8), coin50_50, 2),
-   (1, (5, 9), (coin100_100, 3), coin50_100, 8),
-   (1, (5, 2), (coin100_100, 3), coin50_50, 2),
-   (1, (2, 9), (coin50_50, 2), coin50_100, 8),
-   (1, (2, 5), (coin50_50, 2), coin100_100, 3)
+  have state_nondeterminism_1: "state_nondeterminism 1 {|(2, coin 50 50, 2), (5, coin 100 100, 3), (9, coin 50 100, 8)|} = {|
+   (1, (9, 5), (coin 50 100, 8), coin 100 100, 3),
+   (1, (9, 2), (coin 50 100, 8), coin 50 50, 2),
+   (1, (5, 9), (coin 100 100, 3), coin 50 100, 8),
+   (1, (5, 2), (coin 100 100, 3), coin 50 50, 2),
+   (1, (2, 9), (coin 50 50, 2), coin 50 100, 8),
+   (1, (2, 5), (coin 50 50, 2), coin 100 100, 3)
    |}"
     apply (simp add: state_nondeterminism_def minus_2 minus_3)
     by auto
@@ -662,62 +320,57 @@ proof-
     apply (simp add: nondeterministic_pairs_def S_def merged_1_8_def)
     apply (simp add: outgoing_transitions_def fimage_def state_nondeterminsm_0 state_nondeterminism_1)
     apply (simp add: ffilter_def fset_both_sides Abs_fset_inverse Set.filter_def)
-    apply safe
-    by (simp_all add: choices orders)
+    by auto
 qed
 
 lemma nondeterministic_pairs_merged_1_7: "nondeterministic_pairs merged_1_7 = {|
-(1, (2, 8), (coin50_50, 2), coin50_50, 7),
-(1, (8, 2), (coin50_50, 7), coin50_50, 2)
+(1, (2, 8), (coin 50 50, 2), coin 50 50, 7),
+(1, (8, 2), (coin 50 50, 7), coin 50 50, 2)
 |}"
 proof-
-  have minus_1: "{(2, coin50_50, 2), (5, coin100_100, 3), (8, coin50_50, 7)} - {(5, coin100_100, 3)} = {(2, coin50_50, 2), (8, coin50_50, 7)}"
-    apply (simp add: transitions)
+  have minus_1: "{(2, coin 50 50, 2), (5, coin 100 100, 3), (8, coin 50 50, 7)} - {(5, coin 100 100, 3)} = {(2, coin 50 50, 2), (8, coin 50 50, 7)}"
     by auto
-  have minus_2: "{(2, coin50_50, 2::nat), (5, coin100_100, 3), (8, coin50_50, 7)} - {(8, coin50_50, 7)} = {(2, coin50_50, 2), (5, coin100_100, 3)}"
-    apply (simp add: transitions)
+  have minus_2: "{(2, coin 50 50, 2::nat), (5, coin 100 100, 3), (8, coin 50 50, 7)} - {(8, coin 50 50, 7)} = {(2, coin 50 50, 2), (5, coin 100 100, 3)}"
     by auto
-  have state_nondeterminism_1: "state_nondeterminism 1 {|(2, coin50_50, 2), (5, coin100_100, 3), (8, coin50_50, 7)|} = {|
-      (1, (8, 5), (coin50_50, 7), coin100_100, 3),
-      (1, (8, 2), (coin50_50, 7), coin50_50, 2),
-      (1, (5, 8), (coin100_100, 3), coin50_50, 7),
-      (1, (5, 2), (coin100_100, 3), coin50_50, 2),
-      (1, (2, 8), (coin50_50, 2), coin50_50, 7),
-      (1, (2, 5), (coin50_50, 2), coin100_100, 3)
+  have state_nondeterminism_1: "state_nondeterminism 1 {|(2, coin 50 50, 2), (5, coin 100 100, 3), (8, coin 50 50, 7)|} = {|
+      (1, (8, 5), (coin 50 50, 7), coin 100 100, 3),
+      (1, (8, 2), (coin 50 50, 7), coin 50 50, 2),
+      (1, (5, 8), (coin 100 100, 3), coin 50 50, 7),
+      (1, (5, 2), (coin 100 100, 3), coin 50 50, 2),
+      (1, (2, 8), (coin 50 50, 2), coin 50 50, 7),
+      (1, (2, 5), (coin 50 50, 2), coin 100 100, 3)
     |}"
     apply (simp add: state_nondeterminism_def fimage_def minus_1 minus_2)
     by auto
-  have minus_3: "{(1, selectCoke, 0), (1, selectPepsi, 1)} - {(1, selectPepsi, 1)} = {(1, selectCoke, 0)}"
-    apply (simp add: transitions Str_coke Str_pepsi)
+  have minus_3: "{(1, select coke, 0), (1, select pepsi, 1)} - {(1, select pepsi, 1)} = {(1, select coke, 0)}"
     by auto
-  have state_nondeterminism_0: "state_nondeterminism 0 {|(1, selectCoke, 0), (1, selectPepsi, 1)|} = {|(0, (1, 1), (selectPepsi, 1), selectCoke, 0), (0, (1, 1), (selectCoke, 0), selectPepsi, 1)|}"
+  have state_nondeterminism_0: "state_nondeterminism 0 {|(1, select coke, 0), (1, select pepsi, 1)|} = {|(0, (1, 1), (select pepsi, 1), select coke, 0), (0, (1, 1), (select coke, 0), select pepsi, 1)|}"
     by (simp add: state_nondeterminism_def fimage_def minus_3)
   show ?thesis
     apply (simp add: nondeterministic_pairs_def S_def merged_1_7_def)
     apply (simp add: outgoing_transitions_def fimage_def state_nondeterminism_1 state_nondeterminism_0)
     apply (simp add: ffilter_def fset_both_sides Abs_fset_inverse)
     apply (simp add: Set.filter_def)
-    apply safe
-    by (simp_all add: choices)
+    by auto
 qed
 
 definition generator :: generator_function where
-  "generator oldEFSM t1FromOld t1 t2FromOld t2 = (if (oldEFSM, t1FromOld, t1, t2FromOld, t2) = (pta, 1, coin50_50, 8, coin50_100) then None
+  "generator oldEFSM t1FromOld t1 t2FromOld t2 = (if (oldEFSM, t1FromOld, t1, t2FromOld, t2) = (pta, 1, coin 50 50, 8, coin 50 100) then None
                                                   else None)"
 
 definition merged_1_3 :: iEFSM where
-  "merged_1_3 = {|(0, (0, 1), selectGeneral), (2, (1, 1), coin50_50), (4, (1, 1), coin50_100), (5, (1, 4), vend_general),
-                                              (3, (1, 5), coin100_100), (6, (5, 6), vend_general)|}"
+  "merged_1_3 = {|(0, (0, 1), selectGeneral), (2, (1, 1), coin 50 50), (4, (1, 1), coin 50 100), (5, (1, 4), vend_general),
+                                              (3, (1, 5), coin 100 100), (6, (5, 6), vend_general)|}"
 
 definition selectGeneral_2 :: transition where
   "selectGeneral_2 = \<lparr>Label = (STR ''select''), Arity = 1, Guard = [], Outputs = [], Updates = [(R 1, V (I 1)), (R 2, (L (Num 0)))]\<rparr>"
 
 definition merged_1_3_coin :: iEFSM where
   "merged_1_3_coin = {|(0, (0, 1), selectGeneral_2), (2, (1, 1), coinGeneral), (5, (1, 4), vend_general),
-                                              (3, (1, 5), coin100_100), (6, (5, 6), vend_general)|}"
+                                              (3, (1, 5), coin 100 100), (6, (5, 6), vend_general)|}"
 
 definition merged_1_5 :: iEFSM where
-  "merged_1_5 = {|(0, (0, 1), selectGeneral_2), (2, (1, 1), coinGeneral), (5, (1, 4), vend_general), (3, (1, 1), coin100_100),
+  "merged_1_5 = {|(0, (0, 1), selectGeneral_2), (2, (1, 1), coinGeneral), (5, (1, 4), vend_general), (3, (1, 1), coin 100 100),
       (6, (1, 6), vend_general)|}"
 
 definition merged_1_5_coin :: iEFSM where
@@ -736,197 +389,66 @@ lemma set_nequiv_def: "(s \<noteq> s') = (\<exists>e. (e \<in> s \<and> e \<noti
    apply simp
   by simp
 
-lemma coin50_50_cant_directly_subsume_coin50_100: "\<not> directly_subsumes e t s coin50_50 coin50_100"
-    using no_subsumption_coin50_50_coin50_100 cant_directly_subsume
-    by simp
+lemma coin_50_50_cant_directly_subsume_coin_50_100: "\<not> directly_subsumes e t s (coin 50 50) (coin 50 100)"
+  by (simp add: directly_subsumes_def subsumes_def)
 
-lemma coin50_100_cant_directly_subsume_coin50_50: "\<not> directly_subsumes e t s coin50_100 coin50_50"
-    using no_subsumption_coin50_100_coin50_50 cant_directly_subsume
-    by simp
-
-lemma cant_merge_coins: "merge_transitions pta merged_2_9 8 1 1 2 2 coin50_100 8 coin50_50 2 generator modifier True = None"
-proof-
-  have modify_none: "modifier 8 2 1 merged_2_9 pta = None"
-    by eval
-  show ?thesis
-    apply (simp add: merge_transitions_def easy_merge_def modify_none generator_def)
-    apply (simp add: coin50_100_cant_directly_subsume_coin50_50)
-    by (simp add: coin50_50_cant_directly_subsume_coin50_100)
-qed
-
-lemma cant_merge_coins_2: "merge_transitions pta (merge_states (arrives 2 merged_1_8) (arrives 8 merged_1_8) merged_1_8) (leaves 2 pta) (leaves 8 pta)
-           (leaves 2 (merge_states (arrives 2 merged_1_8) (arrives 8 merged_1_8) merged_1_8))
-           (arrives 2 (merge_states (arrives 2 merged_1_8) (arrives 8 merged_1_8) merged_1_8))
-           (arrives 8 (merge_states (arrives 2 merged_1_8) (arrives 8 merged_1_8) merged_1_8)) coin50_50 2 coin50_100 8 generator modifier
-           True = None"
-proof-
-  have modify_none: "modifier 2 8 (leaves 2 (merge_states (arrives 2 merged_1_8) (arrives 8 merged_1_8) merged_1_8))
-             (merge_states (arrives 2 merged_1_8) (arrives 8 merged_1_8) merged_1_8) pta = None"
-    by (simp add: modifier_def transitions)
-  show ?thesis
-    apply (simp add: merge_transitions_def easy_merge_def generator_def modify_none)
-    apply (simp add: coin50_50_cant_directly_subsume_coin50_100)
-    by (simp add: coin50_100_cant_directly_subsume_coin50_50)
-qed
-
-lemma merge_1_8: "merge pta 1 8 generator modifier = None"
-proof-
-  have leaves_2_pta: "leaves 2 pta = 1"
-  proof-
-    have set_filter: "Set.filter (\<lambda>x. \<exists>a b ba. x = (2, (a, b), ba)) (fset pta) = {(2, (1, 2), coin50_50)}"
-      apply (simp add: Set.filter_def pta_def)
-      apply safe
-      by (simp_all add: transitions)
-    show ?thesis
-      by (simp add: leaves_def ffilter_def fthe_elem_def Abs_fset_inverse set_filter)
-  qed
-  have leaves_1_8_pta: "leaves 8 pta = 8"
-  proof-
-    have set_filter: "Set.filter (\<lambda>x. \<exists>a b ba. x = (8, (a, b), ba)) (fset pta) = {(8, (8, 9), coin50_100)}"
-      apply (simp add: Set.filter_def pta_def)
-      apply safe
-      by (simp_all add: transitions)
-    show ?thesis
-      by (simp add: leaves_def ffilter_def fthe_elem_def Abs_fset_inverse set_filter)
-  qed
-  have merged_2_9_neq_merged_1_3: "merged_2_9 \<noteq> merged_1_3"
-    apply (simp add: merged_2_9_def merged_1_3_def set_equiv)
-    apply (simp only: set_nequiv_def)
-    apply (rule_tac x="(0, (0, 1), selectCoke)" in exI)
-    by (simp add: transitions selectGeneral_def)
-  have coin50_50_neq_coinGeneral:  "coin50_50 \<noteq> coinGeneral"
-    by (simp add: coin50_50_def coinGeneral_def)
-  have merge_transitions: "merge_transitions pta merged_2_9 1 8 1 2 2 coin50_50 2 coin50_100 8 generator modifier True = None"
-    apply (simp add: merge_transitions_def easy_merge_def)
-    by (simp add: generator_def modifier_def coin50_50_cant_directly_subsume_coin50_100 coin50_50_neq_coinGeneral
-                     coin50_100_cant_directly_subsume_coin50_50 merged_2_9_neq_merged_1_3)
-  have arrives_2_merged_1_8: "arrives 2 merged_1_8 = 2"
-  proof-
-    have ffilter: "ffilter (\<lambda>x. \<exists>a b ba. x = (2, (a, b), ba)) merged_1_8 = {|(2, (1, 2), coin50_50)|}"
-      apply (simp add: ffilter_def fset_both_sides Abs_fset_inverse merged_1_8_def Set.filter_def)
-      apply safe
-      by (simp_all add: transitions)
-    show ?thesis
-      by (simp add: arrives_def ffilter)
-  qed
-  have arrives_8_merged_1_8: "arrives 8 merged_1_8 = 9"
-  proof-
-    have ffilter: "ffilter (\<lambda>x. \<exists>a b ba. x = (8, (a, b), ba)) merged_1_8 = {|(8, (1, 9), coin50_100)|}"
-      apply (simp add: ffilter_def fset_both_sides Abs_fset_inverse merged_1_8_def Set.filter_def)
-      apply safe
-      by (simp_all add: transitions)
-    show ?thesis
-      by (simp add: arrives_def ffilter)
-  qed
-  have leaves_2_merged_2_9: "leaves 2 merged_2_9 = 1"
-  proof-
-    have ffilter: "ffilter (\<lambda>x. \<exists>a b ba. x = (2, (a, b), ba)) merged_2_9 = {|(2, (1, 2), coin50_50)|}"
-      apply (simp add: ffilter_def merged_2_9_def fset_both_sides Abs_fset_inverse Set.filter_def)
-      apply safe
-      by (simp_all add: transitions)
-    show ?thesis
-      by (simp add: leaves_def ffilter)
-  qed
-  have arrives_2_merged_2_9: "arrives 2 merged_2_9 = 2"
-      proof-
-    have ffilter: "ffilter (\<lambda>x. \<exists>a b ba. x = (2, (a, b), ba)) merged_2_9 = {|(2, (1, 2), coin50_50)|}"
-      apply (simp add: ffilter_def merged_2_9_def fset_both_sides Abs_fset_inverse Set.filter_def)
-      apply safe
-      by (simp_all add: transitions)
-    show ?thesis
-      by (simp add: arrives_def ffilter)
-  qed
-  have arrives_8_merged_2_9: "arrives 8 merged_2_9 = 2 \<and> leaves 8 merged_2_9 = 1"
-  proof-
-    have ffilter: "ffilter (\<lambda>x. \<exists>a b ba. x = (8, (a, b), ba)) merged_2_9 = {|(8, (1, 2), coin50_100)|}"
-      apply (simp add: ffilter_def merged_2_9_def fset_both_sides Abs_fset_inverse Set.filter_def)
-      apply safe
-      by (simp_all add: transitions) 
-    show ?thesis
-      by (simp add: leaves_def arrives_def ffilter)
-  qed
-  show ?thesis
-    apply (simp add: merge_def merge_states_1_8 nondeterminism_def nondeterministic_pairs_merged_1_8)
-    apply (simp add: sorted_list_of_fset_def)
-    apply (simp add: leaves_2_pta leaves_1_8_pta merge_transitions arrives_8_merged_1_8 arrives_2_merged_1_8)
-    apply (simp add: merge_states_2_9 leaves_2_merged_2_9 arrives_2_merged_2_9 arrives_8_merged_2_9)
-    apply (simp add: cant_merge_coins max_def Let_def cant_merge_coins_2)
-    by (simp add: merge_transitions nondeterminism_def nondeterministic_pairs_merged_1_8)
-qed
+lemma coin_50_100_cant_directly_subsume_coin_50_50: "\<not> directly_subsumes e t s (coin 50 100) (coin 50 50)"
+  by (simp add: directly_subsumes_def subsumes_def)
 
 definition merged_3_9 :: iEFSM where
-  "merged_3_9 = {|(0, (0, 1), selectCoke),  (7, (1, 2), coin50_50),   (8, (2, 3), coin50_100), (5, (3, 4), vend_coke),
-                         (1, (0, 1), selectPepsi), (3, (1, 5), coin100_100), (6, (5, 6), vend_coke),
-                                                   (4, (2, 3), coin50_100),  (9, (3, 10), vend_pepsi)|}"
+  "merged_3_9 = {|(0, (0, 1), select coke),  (7, (1, 2), coin 50 50),   (8, (2, 3), coin 50 100), (5, (3, 4), (vend coke)),
+                         (1, (0, 1), select pepsi), (3, (1, 5), coin 100 100), (6, (5, 6), (vend coke)),
+                                                   (4, (2, 3), coin 50 100),  (9, (3, 10), (vend pepsi))|}"
 
 definition merged_3_9_coin100 :: iEFSM where
-  "merged_3_9_coin100 = {|(0, (0, 1), selectCoke),  (7, (1, 2), coin50_50),  (5, (3, 4), vend_coke),
-                         (1, (0, 1), selectPepsi), (3, (1, 5), coin100_100), (6, (5, 6), vend_coke),
-                                                   (8, (2, 3), coin50_100),  (9, (3, 10), vend_pepsi)|}"
+  "merged_3_9_coin100 = {|(0, (0, 1), select coke),  (7, (1, 2), coin 50 50),  (5, (3, 4), (vend coke)),
+                         (1, (0, 1), select pepsi), (3, (1, 5), coin 100 100), (6, (5, 6), (vend coke)),
+                                                   (8, (2, 3), coin 50 100),  (9, (3, 10), (vend pepsi))|}"
 
-lemma consistent_medial_medial_coin50: "and (if r = V (I 1) then snd (V (I 1), cexp.Eq (Num 50)) else cexp.Bc True)
-             (and (if r = V (I 1) then snd (V (I 1), cexp.Eq (Num 50)) else cexp.Bc True) (c r)) =
-            Undef \<or>
-            gval
-             (cexp2gexp r
-               (and (if r = V (I 1) then snd (V (I 1), cexp.Eq (Num 50)) else cexp.Bc True)
-                 (and (if r = V (I 1) then snd (V (I 1), cexp.Eq (Num 50)) else cexp.Bc True) (c r))))
-             s =
-            Some True \<Longrightarrow>
-    (r = V (I 1) \<longrightarrow>
-             and (cexp.Eq (Num 50)) (c (V (I 1))) = Undef \<or>
-             gval (cexp2gexp (V (I 1)) (and (cexp.Eq (Num 50)) (c (V (I 1))))) s = Some True) \<and>
-            (r \<noteq> V (I 1) \<longrightarrow> c r = Undef \<or> gval (cexp2gexp r (c r)) s = Some True)"
-  apply (case_tac "c (V (I 1))")
-        apply auto[1]
-       apply simp
-       apply (case_tac x2)
-        apply auto[1]
-       apply auto[1]
-      apply auto[1]
-     apply (case_tac "MaybeBoolInt (\<lambda>x y. y < x) (Some x4) (s (I 1))")
-      apply auto[1]
-     apply auto[1]
-    apply (case_tac "MaybeBoolInt (\<lambda>x y. y < x) (s (I 1)) (Some x5)")
-     apply auto[1]
-    apply auto[1]
-   apply (case_tac "gval (cexp2gexp (V (I 1)) x6) s")
-    apply auto[1]
-   apply auto[1]
-  apply (case_tac "gval (cexp2gexp (V (I 1)) x71) s")
-   apply auto[1]
-  apply (case_tac "gval (cexp2gexp (V (I 1)) x72) s")
-  by auto
+lemma ctx_simp: "(\<lambda>r. and (if r = V (I 1) then snd (V (I 1), cexp.Eq (Num 50)) else cexp.Bc True) (c r)) = 
+       (\<lambda>r. if r = V (I 1) then and (Eq (Num 50)) (c r) else (c r))"
+  apply (rule ext)
+  by simp
 
-lemma subsumes_coin50_50_coin50_50: "subsumes c coin50_50 coin50_50"
+lemma ctx_simp_2: "(\<lambda>r. and (if r = V (I 1) then snd (V (I 1), cexp.Eq (Num m)) else cexp.Bc True)
+           (and (if r = V (I 1) then snd (V (I 1), cexp.Eq (Num m)) else cexp.Bc True) (c r))) = 
+(\<lambda>r. if r = V (I 1) then and (Eq (Num m)) (and (Eq (Num m)) (c r)) else c r)"
+  apply (rule ext)
+  by simp
+
+lemma cval_false_eq_undef: "\<forall>r i. cval (Bc False) i = cval (Undef) i"
+  by simp
+
+lemma ctx_simp_3: "(\<lambda>r. and (if r = V (I 1) then snd (V (I 1), cexp.Eq (Num m)) else cexp.Bc True) (c r)) =
+       (\<lambda>r. (if r = V (I 1) then and (cexp.Eq (Num m)) (c r) else c r))"
+  apply (rule ext)
+  by simp
+
+lemma "consistent
+     (\<lambda>r. and (if r = V (I 1) then snd (V (I 1), cexp.Eq (Num m)) else cexp.Bc True)
+           (and (if r = V (I 1) then snd (V (I 1), cexp.Eq (Num m)) else cexp.Bc True) (c r))) \<Longrightarrow>
+    consistent (\<lambda>r. and (if r = V (I 1) then snd (V (I 1), cexp.Eq (Num m)) else cexp.Bc True) (c r))"
+  apply (simp add: ctx_simp_2 ctx_simp_3)
+  apply (simp add: consistent_def)
+  oops
+
+lemma subsumes_coin_50_50_coin_50_50: "subsumes c (coin m n) (coin m n)"
 proof-
-  have consistent: "consistent
-          (\<lambda>r. and (if r = V (I 1) then snd (V (I 1), cexp.Eq (Num 50)) else cexp.Bc True)
-                (and (if r = V (I 1) then snd (V (I 1), cexp.Eq (Num 50)) else cexp.Bc True) (c r))) \<Longrightarrow>
-         consistent (\<lambda>r. and (if r = V (I 1) then snd (V (I 1), cexp.Eq (Num 50)) else cexp.Bc True) (c r))"
-    apply (simp add: consistent_def)
-    using consistent_medial_medial_coin50
-    by blast
   show ?thesis
-  apply (simp add: subsumes_def coin50_50_def posterior_def)
-  apply (case_tac "consistent (\<lambda>r. and (if r = V (I 1) then snd (V (I 1), cexp.Eq (Num 50)) else cexp.Bc True)
-                           (and (if r = V (I 1) then snd (V (I 1), cexp.Eq (Num 50)) else cexp.Bc True) (c r)))")
-   apply (simp add: remove_input_constraints_def)
-   apply clarify
-   apply (case_tac "r = V (I 1)")
-    apply simp
-    apply (case_tac "consistent (\<lambda>r. and (if r = V (I 1) then snd (V (I 1), cexp.Eq (Num 50)) else cexp.Bc True) (c r))")
-     apply (simp add: remove_input_constraints_def)
+  apply (simp add: subsumes_def)
+  apply (simp add: posterior_def Let_def remove_input_constraints_def ctx_simp)
+    apply clarify
+    apply standard
+     apply clarify
+     apply (case_tac "cval (c r) i")
       apply simp
-      apply (simp add: consistent)
      apply simp
-     apply (case_tac "consistent (\<lambda>r. and (if r = V (I 1) then snd (V (I 1), cexp.Eq (Num 50)) else cexp.Bc True) (c r))")
-      apply (simp add: remove_input_constraints_def option.case_eq_if)
-    using consistent apply blast
-    by simp
-qed
+    apply clarify
+    apply standard
+     apply clarify
+     apply simp
 
-lemma subsumes_coin50_100_coin50_100: "subsumes c coin50_100 coin50_100"
+lemma subsumes_coin 50 100_coin 50 100: "subsumes c coin 50 100 coin 50 100"
 proof-
   have consistent: "consistent
           (\<lambda>r. and (if r = V (I 1) then snd (V (I 1), cexp.Eq (Num 50)) else cexp.Bc True)
@@ -936,7 +458,7 @@ proof-
     using consistent_medial_medial_coin50
     by blast
   show ?thesis
-  apply (simp add: subsumes_def coin50_100_def posterior_def)
+  apply (simp add: subsumes_def coin 50 100_def posterior_def)
   apply (case_tac "consistent (\<lambda>r. and (if r = V (I 1) then snd (V (I 1), cexp.Eq (Num 50)) else cexp.Bc True)
                            (and (if r = V (I 1) then snd (V (I 1), cexp.Eq (Num 50)) else cexp.Bc True) (c r)))")
    apply (simp add: remove_input_constraints_def)
@@ -956,28 +478,28 @@ qed
 
 definition merged_2_8_coin50 :: iEFSM where
   "merged_2_8_coin50 = {|
-   (9, (9, 10), vend_pepsi),
-   (8, (2, 9), coin50_100),
-   (1, (0, 1), selectPepsi),
-   (6, (5, 6), vend_coke),
-   (3, (1, 5), coin100_100),
-   (5, (3, 4), vend_coke),
-   (4, (2, 3), coin50_100),
-   (0, (0, 1), selectCoke),
-   (7, (1, 2), coin50_50)
+   (9, (9, 10), (vend pepsi)),
+   (8, (2, 9), coin 50 100),
+   (1, (0, 1), select pepsi),
+   (6, (5, 6), (vend coke)),
+   (3, (1, 5), coin 100 100),
+   (5, (3, 4), (vend coke)),
+   (4, (2, 3), coin 50 100),
+   (0, (0, 1), select coke),
+   (7, (1, 2), coin 50 50)
 |}"
 
-lemma replace_coin50: "replace_transition merged_2_8 7 1 2 coin50_50 coin50_50 = merged_2_8_coin50"
+lemma replace_coin50: "replace_transition merged_2_8 7 1 2 coin 50 50 coin 50 50 = merged_2_8_coin50"
 proof-
-  have filter: "{a \<in> fset merged_2_8. snd a \<noteq> ((1, 2), coin50_50)} = {
-   (9, (9, 10), vend_pepsi),
-   (8, (2, 9), coin50_100),
-   (1, (0, 1), selectPepsi),
-   (6, (5, 6), vend_coke),
-   (3, (1, 5), coin100_100),
-   (5, (3, 4), vend_coke),
-   (4, (2, 3), coin50_100),
-   (0, (0, 1), selectCoke)}"
+  have filter: "{a \<in> fset merged_2_8. snd a \<noteq> ((1, 2), coin 50 50)} = {
+   (9, (9, 10), (vend pepsi)),
+   (8, (2, 9), coin 50 100),
+   (1, (0, 1), select pepsi),
+   (6, (5, 6), (vend coke)),
+   (3, (1, 5), coin 100 100),
+   (5, (3, 4), (vend coke)),
+   (4, (2, 3), coin 50 100),
+   (0, (0, 1), select coke)}"
     apply (simp add: merged_2_8_def)
     apply standard
      apply clarify
@@ -1004,24 +526,24 @@ proof-
     by auto
 qed
 
-lemma nondeterministic_pairs_merged_2_8_coin50: "nondeterministic_pairs merged_2_8_coin50 = {|(2, (3, 9), (coin50_100, 4), coin50_100, 8), (2, (9, 3), (coin50_100, 8), coin50_100, 4)|}"
+lemma nondeterministic_pairs_merged_2_8_coin50: "nondeterministic_pairs merged_2_8_coin50 = {|(2, (3, 9), (coin 50 100, 4), coin 50 100, 8), (2, (9, 3), (coin 50 100, 8), coin 50 100, 4)|}"
 proof-
-  have minus_1: "{|(5, coin100_100, 3), (2, coin50_50, 2)|} |-| {|(2, coin50_50, 2)|} = {|(5, coin100_100, 3)|}"
-    apply (simp add: transitions)
+  have minus_1: "{|(5, coin 100 100, 3), (2, coin 50 50, 2)|} |-| {|(2, coin 50 50, 2)|} = {|(5, coin 100 100, 3)|}"
+    apply simp
     by auto
-  have minus_3: "{(1, selectCoke, 0), (1, selectPepsi, 1)} - {(1, selectPepsi, 1)} = {(1, selectCoke, 0)}"
-    apply (simp add: transitions Str_coke Str_pepsi)
+  have minus_3: "{(1, select coke, 0), (1, select pepsi, 1)} - {(1, select pepsi, 1)} = {(1, select coke, 0)}"
+    apply (simp add: Str_coke Str_pepsi)
     by auto
-  have minus_2: "{|(9, coin50_100, 8::nat), (3, coin50_100, 4)|} |-| {|(3, coin50_100, 4)|} = {|(9, coin50_100, 8)|}"
-    apply (simp add: transitions)
+  have minus_2: "{|(9, coin 50 100, 8::nat), (3, coin 50 100, 4)|} |-| {|(3, coin 50 100, 4)|} = {|(9, coin 50 100, 8)|}"
+    apply simp
     by auto
-  have state_nondeterminism_0: "state_nondeterminism 0 {|(1, selectCoke, 0), (1, selectPepsi, 1)|} = {|(0, (1, 1), (selectPepsi, 1), selectCoke, 0), (0, (1, 1), (selectCoke, 0), selectPepsi, 1)|}"
+  have state_nondeterminism_0: "state_nondeterminism 0 {|(1, select coke, 0), (1, select pepsi, 1)|} = {|(0, (1, 1), (select pepsi, 1), select coke, 0), (0, (1, 1), (select coke, 0), select pepsi, 1)|}"
     by (simp add: state_nondeterminism_def fimage_def minus_3)
-  have outgoing_0_equiv: "{|(1, selectPepsi, 1), (1, selectCoke, 0)|} = {|(1, selectCoke, 0), (1, selectPepsi, 1)|}"
+  have outgoing_0_equiv: "{|(1, select pepsi, 1), (1, select coke, 0)|} = {|(1, select coke, 0), (1, select pepsi, 1)|}"
     by auto
-  have state_nondeterminism_1: "state_nondeterminism 1 {|(5, coin100_100, 3), (2, coin50_50, 7)|} = {|(1, (2, 5), (coin50_50, 7), coin100_100, 3), (1, (5, 2), (coin100_100, 3), coin50_50, 7)|}"
+  have state_nondeterminism_1: "state_nondeterminism 1 {|(5, coin 100 100, 3), (2, coin 50 50, 7)|} = {|(1, (2, 5), (coin 50 50, 7), coin 100 100, 3), (1, (5, 2), (coin 100 100, 3), coin 50 50, 7)|}"
     by eval
-  have state_nondeterminism_2: "state_nondeterminism 2 {|(9, coin50_100, 8), (3, coin50_100, 4)|} = {|(2, (3, 9), (coin50_100, 4), coin50_100, 8), (2, (9, 3), (coin50_100, 8), coin50_100, 4)|}"
+  have state_nondeterminism_2: "state_nondeterminism 2 {|(9, coin 50 100, 8), (3, coin 50 100, 4)|} = {|(2, (3, 9), (coin 50 100, 4), coin 50 100, 8), (2, (9, 3), (coin 50 100, 8), coin 50 100, 4)|}"
     by (simp add: state_nondeterminism_def minus_2)
   show ?thesis
     apply (simp add: nondeterministic_pairs_def S_def merged_2_8_coin50_def)
@@ -1033,24 +555,24 @@ proof-
 qed
 
 lemma nondeterministic_pairs_merged_3_9_coin100: "nondeterministic_pairs merged_3_9_coin100 = {|
-(3, (10, 4), (vend_pepsi, 9), vend_coke, 5), 
-(3, (4, 10), (vend_coke, 5), vend_pepsi, 9)
+(3, (10, 4), ((vend pepsi), 9), (vend coke), 5), 
+(3, (4, 10), ((vend coke), 5), (vend pepsi), 9)
 |}"
 proof-
-  have minus_1: "{|(2, coin50_50, 2), (5, coin100_100, 3)|} |-| {|(5, coin100_100, 3)|} = {|(2, coin50_50, 2)|}"
-    apply (simp add: transitions)
+  have minus_1: "{|(2, coin 50 50, 2), (5, coin 100 100, 3)|} |-| {|(5, coin 100 100, 3)|} = {|(2, coin 50 50, 2)|}"
+    apply simp
     by auto
-  have minus_2: "{|(4, vend_coke, 5), (10, vend_pepsi, 9)|} |-| {|(10, vend_pepsi, 9)|} = {|(4, vend_coke, 5)|}"
-    apply (simp add: transitions Str_coke Str_pepsi)
+  have minus_2: "{|(4, (vend coke), 5), (10, (vend pepsi), 9)|} |-| {|(10, (vend pepsi), 9)|} = {|(4, (vend coke), 5)|}"
+    apply (simp add: Str_coke Str_pepsi)
     by auto
-  have minus_3: "{(1, selectCoke, 0), (1, selectPepsi, 1)} - {(1, selectPepsi, 1)} = {(1, selectCoke, 0)}"
-    apply (simp add: transitions Str_coke Str_pepsi)
+  have minus_3: "{(1, select coke, 0), (1, select pepsi, 1)} - {(1, select pepsi, 1)} = {(1, select coke, 0)}"
+    apply (simp add: Str_coke Str_pepsi)
     by auto
-  have state_nondeterminism_0: "state_nondeterminism 0 {|(1, selectCoke, 0), (1, selectPepsi, 1)|} = {|(0, (1, 1), (selectPepsi, 1), selectCoke, 0), (0, (1, 1), (selectCoke, 0), selectPepsi, 1)|}"
+  have state_nondeterminism_0: "state_nondeterminism 0 {|(1, select coke, 0), (1, select pepsi, 1)|} = {|(0, (1, 1), (select pepsi, 1), select coke, 0), (0, (1, 1), (select coke, 0), select pepsi, 1)|}"
     by (simp add: state_nondeterminism_def fimage_def minus_3)
-  have state_nondeterminism_1: "state_nondeterminism 1 {|(2, coin50_50, 7), (5, coin100_100, 3)|} = {|(1, (5, 2), (coin100_100, 3), coin50_50, 7), (1, (2, 5), (coin50_50, 7), coin100_100, 3)|}"
+  have state_nondeterminism_1: "state_nondeterminism 1 {|(2, coin 50 50, 7), (5, coin 100 100, 3)|} = {|(1, (5, 2), (coin 100 100, 3), coin 50 50, 7), (1, (2, 5), (coin 50 50, 7), coin 100 100, 3)|}"
     by eval
-  have state_nondeterminism_3: "state_nondeterminism 3 {|(4, vend_coke, 5), (10, vend_pepsi, 9)|} = {|(3, (10, 4), (vend_pepsi, 9), vend_coke, 5), (3, (4, 10), (vend_coke, 5), vend_pepsi, 9)|}"
+  have state_nondeterminism_3: "state_nondeterminism 3 {|(4, (vend coke), 5), (10, (vend pepsi), 9)|} = {|(3, (10, 4), ((vend pepsi), 9), (vend coke), 5), (3, (4, 10), ((vend coke), 5), (vend pepsi), 9)|}"
     by (simp add: state_nondeterminism_def minus_2)
   show ?thesis
     apply (simp add: nondeterministic_pairs_def S_def merged_3_9_coin100_def)
@@ -1085,7 +607,7 @@ qed
 lemma possible_steps_not_vend: "aa = (STR ''vend'') \<longrightarrow> b \<noteq> [] \<Longrightarrow> possible_steps (tm pta) 3 Map.empty aa b = {||}"
   apply (simp add: possible_steps_fst)
   apply (simp add: tm_def pta_def Set.filter_def)
-  apply (simp add: vend_coke_def)
+  apply (simp add: (vend coke)_def)
   by auto
 
 lemma nondetermnistic_step_not_vend: "aa = (STR ''vend'') \<longrightarrow> b \<noteq> [] \<Longrightarrow> nondeterministic_step (tm pta) 3 Map.empty aa b = None"
@@ -1095,7 +617,7 @@ lemma possible_steps_vend: "possible_steps (tm merged_vends) 3 r (STR ''vend'') 
   apply (simp add: possible_steps_fst)
   apply (simp add: tm_def merged_vends_def Set.filter_def)
   apply safe
-           apply (simp_all add: transitions selectGeneral_def vend_general_def)
+           apply (simp_all add: selectGeneral_def vend_general_def)
   by force
 
 lemma nondeterministic_simulates_trace_merged_vends_pta_3_3: "nondeterministic_simulates_trace (tm merged_vends) (tm pta) 3 3 <R 1 := (Str ''coke'')> Map.empty t"
@@ -1126,14 +648,14 @@ qed
 lemma possible_steps_pta_2_not_coin50: "aa = (STR ''coin'') \<longrightarrow> b \<noteq> [Num 50] \<Longrightarrow> possible_steps (tm pta) 2 Map.empty aa b = {||}"
   apply (simp add: possible_steps_fst)
   apply (simp add: Set.filter_def tm_def pta_def)
-  apply (simp add: coin50_100_def hd_input2state)
+  apply (simp add: coin 50 100_def hd_input2state)
   by (metis One_nat_def length_0_conv length_Suc_conv list.sel(1))
 
-lemma possible_steps_merged_vends_coin50_2: "\<forall>r. possible_steps (tm merged_vends) 2 r (STR ''coin'') [Num 50] = {|(3, coin50_100)|}"
+lemma possible_steps_merged_vends_coin50_2: "\<forall>r. possible_steps (tm merged_vends) 2 r (STR ''coin'') [Num 50] = {|(3, coin 50 100)|}"
     apply (simp add: possible_steps_fst)
     apply (simp add: tm_def merged_vends_def Set.filter_def)
     apply safe
-              apply (simp_all add: transitions selectGeneral_def)
+              apply (simp_all add: selectGeneral_def)
     by force
 
 lemma nondeterministic_simulates_trace_merged_vends_pta_2_2: "nondeterministic_simulates_trace (tm merged_vends) (tm pta) 2 2 <R 1 := (Str ''coke'')> Map.empty t"
@@ -1142,10 +664,10 @@ proof(induct t)
   then show ?case
     by (simp add: nondeterministic_simulates_trace.base)
 next
-  have coin50_updates: "\<forall>r. EFSM.apply_updates (Updates coin50_100) (join_ir [Num 50] r) r = r"
+  have coin50_updates: "\<forall>r. EFSM.apply_updates (Updates coin 50 100) (join_ir [Num 50] r) r = r"
     apply clarify
     apply (rule ext)
-    by (simp add: transitions)
+    by (simp add:)
   have regsimp: "(\<lambda>a. if a = R 1 then Some ((Str ''coke'')) else None) = <R 1 := (Str ''coke'')>"
     apply (rule ext)
     by simp
@@ -1157,7 +679,7 @@ next
         apply (simp add: step_nondet_step_equiv step_pta_coin50_2)
        apply (simp add: possible_steps_merged_vends_coin50_2)
        apply (simp only: coin50_updates regsimp)
-      apply (simp add: coin50_100_def)
+      apply (simp add: coin 50 100_def)
      apply (simp add: nondeterministic_simulates_trace_merged_vends_pta_3_3)
     apply (case_tac a)
     apply simp
@@ -1184,7 +706,7 @@ qed
 
 lemma possible_steps_pta_5_not_vend: "a = (STR ''vend'') \<longrightarrow> b \<noteq> [] \<Longrightarrow> possible_steps (tm pta) 5 Map.empty a b = {||}"
   apply (simp add: possible_steps_fst)
-  apply (simp add: tm_def pta_def Set.filter_def vend_coke_def)
+  apply (simp add: tm_def pta_def Set.filter_def (vend coke)_def)
   by force
 
 lemma nondeterministic_simulates_trace_merged_vends_pta_5_5: "nondeterministic_simulates_trace (tm merged_vends) (tm pta) 5 5 <R 1 := (Str ''coke'')> Map.empty t"
@@ -1199,7 +721,7 @@ next
   have possible_steps_vend: "possible_steps (tm merged_vends) 5 <R 1 := (Str ''coke'')> (STR ''vend'') [] = {|(6, vend_general)|}"
     apply (simp add: possible_steps_fst)
     apply (simp add: tm_def merged_vends_def Set.filter_def)
-    apply (simp add: transitions vend_general_def)
+    apply (simp add: vend_general_def)
     by force
   case (Cons a t)
   case (Cons a t)
@@ -1227,24 +749,24 @@ lemma possible_steps_pta_1_not_coin: "aa = (STR ''coin'') \<longrightarrow> b \<
   apply (case_tac "Label baa = (STR ''coin'')")
    apply simp
    apply (case_tac "ba = 2")
-    apply (simp add: transitions hd_input2state)
+    apply (simp add: hd_input2state)
     apply (metis One_nat_def length_0_conv length_Suc_conv list.sel(1))
-   apply (simp add: transitions hd_input2state)
+   apply (simp add: hd_input2state)
    apply (metis One_nat_def length_0_conv length_Suc_conv list.sel(1))
-  by (simp add: transitions)
+  by (simp add:)
 
-lemma possible_steps_merged_vends_coin50_1: "possible_steps (tm merged_vends) 1 r (STR ''coin'') [Num 50] = {|(2, coin50_50)|}"
+lemma possible_steps_merged_vends_coin50_1: "possible_steps (tm merged_vends) 1 r (STR ''coin'') [Num 50] = {|(2, coin 50 50)|}"
     apply (simp add: possible_steps_fst)
     apply (simp add: tm_def merged_vends_def Set.filter_def)
     apply safe
-              apply (simp_all add: transitions selectGeneral_def)
+              apply (simp_all add: selectGeneral_def)
   by force
 
-lemma possible_steps_merged_vends_coin100: "possible_steps (tm merged_vends) 1 r (STR ''coin'') [Num 100] = {|(5, coin100_100)|}"
+lemma possible_steps_merged_vends_coin100: "possible_steps (tm merged_vends) 1 r (STR ''coin'') [Num 100] = {|(5, coin 100 100)|}"
     apply (simp add: possible_steps_fst)
     apply (simp add: tm_def merged_vends_def Set.filter_def)
     apply safe
-              apply (simp_all add: transitions selectGeneral_def vend_general_def)
+              apply (simp_all add: selectGeneral_def vend_general_def)
     by force
 
 lemma nondeterministic_simulates_trace_merged_vends_pta_1_1: "nondeterministic_simulates_trace (tm merged_vends) (tm pta) 1 1 <R 1 := (Str ''coke'')> Map.empty t"
@@ -1253,10 +775,10 @@ proof(induct t)
   then show ?case
     by (simp add: nondeterministic_simulates_trace.base)
 next
-  have coin50_updates: "\<forall>r. EFSM.apply_updates (Updates coin50_50) (join_ir [Num 50] r) r = r"
+  have coin50_updates: "\<forall>r. EFSM.apply_updates (Updates coin 50 50) (join_ir [Num 50] r) r = r"
     apply clarify
     apply (rule ext)
-    by (simp add: transitions)
+    by (simp add:)
   have regsimp: "(\<lambda>a. if a = R 1 then Some ((Str ''coke'')) else None) = <R 1 := (Str ''coke'')>"
     apply (rule ext)
     by simp
@@ -1268,15 +790,15 @@ next
         apply (simp add: step_nondet_step_equiv step_pta_coin50_1)
        apply (simp add: possible_steps_merged_vends_coin50_1)
        apply (simp only: coin50_updates regsimp)
-      apply (simp add: coin50_50_def)
+      apply (simp add: coin 50 50_def)
       apply (simp add: nondeterministic_simulates_trace_merged_vends_pta_2_2)
       apply (case_tac "a=((STR ''coin''), [Num 100])")
        apply (simp add: regsimp)
      apply (rule nondeterministic_simulates_trace.step_some)
          apply (simp add: step_nondet_step_equiv step_pta_coin100_1)
         apply (simp add: possible_steps_merged_vends_coin100)
-       apply (simp add: coin100_100_def)
-      apply (simp add: coin100_100_def)
+       apply (simp add: coin 100 100_def)
+      apply (simp add: coin 100 100_def)
      apply (simp add: nondeterministic_simulates_trace_merged_vends_pta_5_5)
     apply (case_tac a)
     apply (simp add: regsimp)
@@ -1288,7 +810,7 @@ lemma possible_steps_pta_9_not_vend: "aa = (STR ''vend'') \<longrightarrow> b \<
        possible_steps (tm pta) 9 Map.empty aa b = {||}"
   apply (simp add: possible_steps_fst)
   apply (simp add: tm_def pta_def Set.filter_def)
-  apply (simp add: vend_pepsi_def)
+  apply (simp add: (vend pepsi)_def)
   by auto
 
 lemma nondeterministic_simulates_trace_merged_vends_pta_3_9: "nondeterministic_simulates_trace (tm merged_vends) (tm pta) 3 9 <R 1 := (Str ''pepsi'')> Map.empty t"
@@ -1301,7 +823,7 @@ next
     apply (simp add: possible_steps_fst)
     apply (simp add: tm_def merged_vends_def Set.filter_def)
     apply safe
-    apply (simp_all add: transitions vend_general_def)
+    apply (simp_all add: vend_general_def)
     by force
   have possible_steps_10: "\<forall>aaa b. possible_steps (tm pta) 10 Map.empty aaa b = {||}"
     apply (simp add: possible_steps_fst)
@@ -1331,7 +853,7 @@ lemma possible_steps_pta_8_not_coin: "aa = (STR ''coin'') \<longrightarrow> b \<
        possible_steps (tm pta) 8 Map.empty aa b = {||}"
   apply (simp add: possible_steps_fst)
   apply (simp add: tm_def pta_def Set.filter_def)
-  apply (simp add: coin50_100_def hd_input2state)
+  apply (simp add: coin 50 100_def hd_input2state)
   by (metis One_nat_def length_0_conv length_Suc_conv list.sel(1))
 
 lemma nondeterministic_simulates_trace_merged_vends_pta_2_8: "nondeterministic_simulates_trace (tm merged_vends) (tm pta) 2 8 <R 1 := (Str ''pepsi'')> Map.empty t"
@@ -1340,11 +862,11 @@ proof(induct t)
   then show ?case
     by (simp add: nondeterministic_simulates_trace.base)
 next
-  have possible_steps: "possible_steps (tm merged_vends) 2 <R 1 := (Str ''pepsi'')> (STR ''coin'') [Num 50] = {|(3, coin50_100)|}"
+  have possible_steps: "possible_steps (tm merged_vends) 2 <R 1 := (Str ''pepsi'')> (STR ''coin'') [Num 50] = {|(3, coin 50 100)|}"
     apply (simp add: possible_steps_fst)
     apply (simp add: tm_def merged_vends_def Set.filter_def)
     apply safe
-              apply (simp_all add: transitions selectGeneral_def vend_general_def)
+              apply (simp_all add: selectGeneral_def vend_general_def)
     by force
   case (Cons a t)
   have regsimp: "\<forall>d. (\<lambda>a. if a = R 1 then Some d else None) = <R 1 := d>"
@@ -1357,8 +879,8 @@ next
      apply (rule nondeterministic_simulates_trace.step_some)
         apply (simp add: step_nondet_step_equiv step_pta_coin50_8)
        apply (simp add: possible_steps)
-       apply (simp add: coin50_100_def)
-      apply (simp add: coin50_100_def)
+       apply (simp add: coin 50 100_def)
+      apply (simp add: coin 50 100_def)
      apply (simp add: nondeterministic_simulates_trace_merged_vends_pta_3_9)
     apply (case_tac a)
     apply simp
@@ -1369,7 +891,7 @@ qed
 lemma possible_steps_pt_7_not_coin: "aa = (STR ''coin'') \<longrightarrow> b \<noteq> [Num 50] \<Longrightarrow>
        possible_steps (tm pta) 7 Map.empty aa b = {||}"
   apply (simp add: possible_steps_fst)
-  apply (simp add: tm_def pta_def Set.filter_def coin50_50_def hd_input2state)
+  apply (simp add: tm_def pta_def Set.filter_def coin 50 50_def hd_input2state)
   by (metis One_nat_def length_0_conv length_Suc_conv list.sel(1))
 
 lemma nondeterministic_simulates_trace_merged_vends_pta_1_7: "nondeterministic_simulates_trace (tm merged_vends) (tm pta) 1 7 <R 1 := (Str ''pepsi'')> Map.empty t"
@@ -1378,11 +900,11 @@ proof(induct t)
   then show ?case
     by (simp add: nondeterministic_simulates_trace.base)
 next
-  have possible_steps_coin50: "\<forall>r. possible_steps (tm merged_vends) 1 r (STR ''coin'') [Num 50] = {|(2, coin50_50)|}"
+  have possible_steps_coin50: "\<forall>r. possible_steps (tm merged_vends) 1 r (STR ''coin'') [Num 50] = {|(2, coin 50 50)|}"
     apply (simp add: possible_steps_fst)
     apply (simp add: tm_def merged_vends_def Set.filter_def)
     apply safe
-              apply (simp_all add: transitions selectGeneral_def)
+              apply (simp_all add: selectGeneral_def)
     by force
   have regsimp: "\<forall>d. (\<lambda>a. if a = R 1 then Some d else None) = <R 1 := d>"
     apply clarify
@@ -1395,8 +917,8 @@ next
      apply (rule nondeterministic_simulates_trace.step_some)
          apply (simp add: step_nondet_step_equiv step_pta_coin50_7)
         apply (simp add: possible_steps_coin50)
-       apply (simp add: coin50_50_def)
-      apply (simp add: coin50_50_def)
+       apply (simp add: coin 50 50_def)
+      apply (simp add: coin 50 50_def)
      apply (simp add: nondeterministic_simulates_trace_merged_vends_pta_2_8)
     apply (case_tac a)
     apply simp
@@ -1412,9 +934,9 @@ lemma possible_steps_pta_0_not_select: " aa = (STR ''select'') \<longrightarrow>
   apply clarify
   apply simp
   apply (case_tac "ba = 1")
-   apply (simp add: transitions hd_input2state)
+   apply (simp add: hd_input2state)
    apply (metis One_nat_def length_0_conv length_Suc_conv list.sel(1))
-  apply (simp add: transitions hd_input2state)
+  apply (simp add: hd_input2state)
   by (metis One_nat_def length_0_conv length_Suc_conv list.sel(1))
 
 lemma nondeterministic_simulates_trace_merged_vends_pta_0_0: "nondeterministic_simulates_trace (tm merged_vends) (tm pta) 0 0 Map.empty Map.empty t"
@@ -1427,7 +949,7 @@ next
     apply (simp add: possible_steps_fst)
     apply (simp add: tm_def merged_vends_def Set.filter_def)
     apply safe
-              apply (simp_all add: transitions selectGeneral_def)
+              apply (simp_all add: selectGeneral_def)
     by force
   have selectGeneral_updates: "\<forall>d. EFSM.apply_updates (Updates selectGeneral) (join_ir [d] Map.empty) Map.empty = <R 1 := d>"
     apply clarify
@@ -1438,7 +960,7 @@ next
     apply (case_tac "a=((STR ''select''), [(Str ''coke'')])")
      apply simp
      apply (rule nondeterministic_simulates_trace.step_some)
-         apply (simp add: step_nondet_step_equiv step_pta_selectCoke)
+         apply (simp add: step_nondet_step_equiv step_pta_select coke)
         apply (simp add: possible_steps)
        apply (simp only: selectGeneral_updates)
       apply (simp add: selectGeneral_def)
@@ -1446,7 +968,7 @@ next
     apply (case_tac "a=((STR ''select''), [(Str ''pepsi'')])")
      apply simp
      apply (rule nondeterministic_simulates_trace.step_some)
-         apply (simp add: step_nondet_step_equiv step_pta_selectPepsi)
+         apply (simp add: step_nondet_step_equiv step_pta_select pepsi)
         apply (simp add: possible_steps)
        apply (simp only: selectGeneral_updates)
       apply (simp add: selectGeneral_def)
@@ -1459,10 +981,10 @@ qed
 
 lemma nondeterministic_pairs_merged_vends: "nondeterministic_pairs merged_vends = {||}"
 proof-
-  have minus_1: "{|(2, coin50_50, 2), (5, coin100_100, 3)|} |-| {|(5, coin100_100, 3)|} = {|(2, coin50_50, 2)|}"
-    apply (simp add: transitions)
+  have minus_1: "{|(2, coin 50 50, 2), (5, coin 100 100, 3)|} |-| {|(5, coin 100 100, 3)|} = {|(2, coin 50 50, 2)|}"
+    apply simp
     by auto
-  have state_nondeterminism_1: "state_nondeterminism 1 {|(2, coin50_50, 2), (5, coin100_100, 3)|} = {|(1, (5, 2), (coin100_100, 3), coin50_50, 2), (1, (2, 5), (coin50_50, 2), coin100_100, 3)|}"
+  have state_nondeterminism_1: "state_nondeterminism 1 {|(2, coin 50 50, 2), (5, coin 100 100, 3)|} = {|(1, (5, 2), (coin 100 100, 3), coin 50 50, 2), (1, (2, 5), (coin 50 50, 2), coin 100 100, 3)|}"
     by (simp add: state_nondeterminism_def minus_1)
   show ?thesis
     apply (simp add: nondeterministic_pairs_def S_def merged_vends_def)
@@ -1475,91 +997,91 @@ lemma merge_1_7: "merge pta 1 7 generator modifier = Some merged_vends"
 proof-
   have leaves_2_pta: "leaves 2 pta = 1"
   proof-
-    have set_filter: "Set.filter (\<lambda>x. \<exists>a b ba. x = (2, (a, b), ba)) (fset pta) = {(2, (1, 2), coin50_50)}"
+    have set_filter: "Set.filter (\<lambda>x. \<exists>a b ba. x = (2, (a, b), ba)) (fset pta) = {(2, (1, 2), coin 50 50)}"
       apply (simp add: Set.filter_def pta_def)
       apply safe
-      by (simp_all add: transitions)
+      by simp_all
     show ?thesis
       by (simp add: leaves_def ffilter_def fthe_elem_def Abs_fset_inverse set_filter)
   qed
   have leaves_7_pta: "leaves 7 pta = 7"
   proof-
-    have set_filter: "Set.filter (\<lambda>x. \<exists>a b ba. x = (7, (a, b), ba)) (fset pta) = {(7, (7, 8), coin50_50)}"
+    have set_filter: "Set.filter (\<lambda>x. \<exists>a b ba. x = (7, (a, b), ba)) (fset pta) = {(7, (7, 8), coin 50 50)}"
       apply (simp add: Set.filter_def pta_def)
       apply safe
-      by (simp_all add: transitions)
+      by simp_all
     show ?thesis
       by (simp add: leaves_def ffilter_def fthe_elem_def Abs_fset_inverse set_filter)
   qed
   have arrives_2_merged_1_7: "arrives 2 merged_1_7 = 2"
   proof-
-    have ffilter: "ffilter (\<lambda>x. \<exists>a b ba. x = (2, (a, b), ba)) merged_1_7 = {|(2, (1, 2), coin50_50)|}"
+    have ffilter: "ffilter (\<lambda>x. \<exists>a b ba. x = (2, (a, b), ba)) merged_1_7 = {|(2, (1, 2), coin 50 50)|}"
       apply (simp add: ffilter_def merged_1_7_def fset_both_sides Abs_fset_inverse Set.filter_def)
       apply safe
-      by (simp_all add: transitions)
+      by simp_all
     show ?thesis
       by (simp add: arrives_def ffilter)
   qed
   have arrives_7_merged_1_7: "arrives 7 merged_1_7 = 8"
   proof-
-    have ffilter: "ffilter (\<lambda>x. \<exists>a b ba. x = (7, (a, b), ba)) merged_1_7 = {|(7, (1, 8), coin50_50)|}"
+    have ffilter: "ffilter (\<lambda>x. \<exists>a b ba. x = (7, (a, b), ba)) merged_1_7 = {|(7, (1, 8), coin 50 50)|}"
       apply (simp add: ffilter_def merged_1_7_def fset_both_sides Abs_fset_inverse Set.filter_def)
       apply safe
-      by (simp_all add: transitions)
+      by simp_all
     show ?thesis
       by (simp add: arrives_def ffilter)
   qed
-  have directly_subsumes_coin50_coin50: "\<forall>s. directly_subsumes (tm pta) (tm merged_2_8) s coin50_50 coin50_50"
-    by (simp add: directly_subsumes_def subsumes_coin50_50_coin50_50)
-  have easy_merge: "easy_merge pta merged_2_8 7 1 1 2 2 coin50_50 7 coin50_50 2 generator = Some merged_2_8_coin50"
+  have directly_subsumes_coin50_coin50: "\<forall>s. directly_subsumes (tm pta) (tm merged_2_8) s coin 50 50 coin 50 50"
+    by (simp add: directly_subsumes_def subsumes_coin_50_50_coin_50_50)
+  have easy_merge: "easy_merge pta merged_2_8 7 1 1 2 2 coin 50 50 7 coin 50 50 2 generator = Some merged_2_8_coin50"
     unfolding easy_merge_def
     apply (simp add: directly_subsumes_coin50_coin50)
     by (simp add: replace_coin50)
-  have merge_transitions: "merge_transitions pta merged_2_8 7 1 1 2 2 coin50_50 7 coin50_50 2 generator modifier True = Some merged_2_8_coin50"
+  have merge_transitions: "merge_transitions pta merged_2_8 7 1 1 2 2 coin 50 50 7 coin 50 50 2 generator modifier True = Some merged_2_8_coin50"
     apply (simp add: merge_transitions_def)
     by (simp add: easy_merge)
   have leaves_2_merged_2_8: "leaves 2 merged_2_8 = 1"
   proof-
-    have ffilter: "ffilter (\<lambda>x. \<exists>a b ba. x = (2, (a, b), ba)) merged_2_8 = {|(2, (1, 2), coin50_50)|}"
+    have ffilter: "ffilter (\<lambda>x. \<exists>a b ba. x = (2, (a, b), ba)) merged_2_8 = {|(2, (1, 2), coin 50 50)|}"
       apply (simp add: ffilter_def merged_2_8_def fset_both_sides Abs_fset_inverse Set.filter_def)
       apply safe
-      by (simp_all add: transitions)
+      by simp_all
     show ?thesis
       by (simp add: leaves_def ffilter)
   qed
   have arrives_2_merged_2_8: "arrives 2 merged_2_8 = 2"
   proof-
-    have ffilter: "ffilter (\<lambda>x. \<exists>a b ba. x = (2, (a, b), ba)) merged_2_8 = {|(2, (1, 2), coin50_50)|}"
+    have ffilter: "ffilter (\<lambda>x. \<exists>a b ba. x = (2, (a, b), ba)) merged_2_8 = {|(2, (1, 2), coin 50 50)|}"
       apply (simp add: ffilter_def merged_2_8_def fset_both_sides Abs_fset_inverse Set.filter_def)
       apply safe
-      by (simp_all add: transitions)
+      by simp_all
     show ?thesis
       by (simp add: arrives_def ffilter)
   qed
   have arrives_7_merged_2_8: "arrives 7 merged_2_8 = 2"
   proof-
-    have ffilter: "ffilter (\<lambda>x. \<exists>a b ba. x = (7, (a, b), ba)) merged_2_8= {|(7, (1, 2), coin50_50)|}"
+    have ffilter: "ffilter (\<lambda>x. \<exists>a b ba. x = (7, (a, b), ba)) merged_2_8= {|(7, (1, 2), coin 50 50)|}"
       apply (simp add: ffilter_def merged_2_8_def fset_both_sides Abs_fset_inverse Set.filter_def)
       apply safe
-      by (simp_all add: transitions) 
+      by simp_all 
     show ?thesis
       by (simp add: arrives_def ffilter)
   qed
   have arrives_4_merged_2_8_coin50: "arrives 4 merged_2_8_coin50 = 3"
   proof-
-    have ffilter: "ffilter (\<lambda>x. \<exists>a b ba. x = (4, (a, b), ba)) merged_2_8_coin50 = {|(4, (2, 3), coin50_100)|}"
+    have ffilter: "ffilter (\<lambda>x. \<exists>a b ba. x = (4, (a, b), ba)) merged_2_8_coin50 = {|(4, (2, 3), coin 50 100)|}"
       apply (simp add: ffilter_def merged_2_8_coin50_def fset_both_sides Abs_fset_inverse Set.filter_def)
       apply safe
-      by (simp_all add: transitions)
+      by simp_all
     show ?thesis
       by (simp add: arrives_def ffilter)
   qed
   have arrives_8_merged_2_8_coin50: "arrives 8 merged_2_8_coin50 = 9"
   proof-
-    have ffilter: "ffilter (\<lambda>x. \<exists>a b ba. x = (8, (a, b), ba)) merged_2_8_coin50 = {|(8, (2, 9), coin50_100)|}"
+    have ffilter: "ffilter (\<lambda>x. \<exists>a b ba. x = (8, (a, b), ba)) merged_2_8_coin50 = {|(8, (2, 9), coin 50 100)|}"
       apply (simp add: ffilter_def merged_2_8_coin50_def fset_both_sides Abs_fset_inverse Set.filter_def)
       apply safe
-      by (simp_all add: transitions)
+      by simp_all
     show ?thesis
       by (simp add: arrives_def ffilter)
   qed
@@ -1568,64 +1090,64 @@ proof-
     by auto
   have leaves_4_pta: "leaves 4 pta = 2"
   proof-
-    have ffilter: "ffilter (\<lambda>x. \<exists>a b ba. x = (4, (a, b), ba)) pta = {|(4, (2, 3), coin50_100)|}"
+    have ffilter: "ffilter (\<lambda>x. \<exists>a b ba. x = (4, (a, b), ba)) pta = {|(4, (2, 3), coin 50 100)|}"
       apply (simp add: ffilter_def pta_def fset_both_sides Abs_fset_inverse Set.filter_def)
       apply safe
-      by (simp_all add: transitions)
+      by simp_all
     show ?thesis
       by (simp add: leaves_def ffilter)
   qed
   have leaves_8_pta: "leaves 8 pta = 8"
   proof-
-    have ffilter: "ffilter (\<lambda>x. \<exists>a b ba. x = (8, (a, b), ba)) pta = {|(8, (8, 9), coin50_100)|}"
+    have ffilter: "ffilter (\<lambda>x. \<exists>a b ba. x = (8, (a, b), ba)) pta = {|(8, (8, 9), coin 50 100)|}"
       apply (simp add: ffilter_def pta_def fset_both_sides Abs_fset_inverse Set.filter_def)
       apply safe
-      by (simp_all add: transitions)
+      by simp_all
     show ?thesis
       by (simp add: leaves_def ffilter)
   qed
   have leaves_4_merged_3_9: "leaves 4 merged_3_9 = 2 \<and>arrives 4 merged_3_9 = 3"
   proof-
-    have ffilter: "ffilter (\<lambda>x. \<exists>a b ba. x = (4, (a, b), ba)) merged_3_9 = {|(4, (2, 3), coin50_100)|}"
+    have ffilter: "ffilter (\<lambda>x. \<exists>a b ba. x = (4, (a, b), ba)) merged_3_9 = {|(4, (2, 3), coin 50 100)|}"
       apply (simp add: ffilter_def merged_3_9_def fset_both_sides Abs_fset_inverse Set.filter_def)
       apply safe
-      by (simp_all add: transitions)
+      by simp_all
     show ?thesis
       by (simp add: arrives_def leaves_def ffilter)
   qed
   have arrives_8_merged_3_9: "arrives 8 merged_3_9 = 3 \<and> leaves 8 merged_3_9 = 2"
   proof-
-    have ffilter: "ffilter (\<lambda>x. \<exists>a b ba. x = (8, (a, b), ba)) merged_3_9 = {|(8, (2, 3), coin50_100)|}"
+    have ffilter: "ffilter (\<lambda>x. \<exists>a b ba. x = (8, (a, b), ba)) merged_3_9 = {|(8, (2, 3), coin 50 100)|}"
       apply (simp add: ffilter_def merged_3_9_def fset_both_sides Abs_fset_inverse Set.filter_def)
       apply safe
-      by (simp_all add: transitions)
+      by simp_all
     show ?thesis
       by (simp add: leaves_def arrives_def ffilter)
   qed
-  have coin50_100_subsumes_self: "directly_subsumes (tm pta) (tm merged_3_9) 2 coin50_100 coin50_100"
-    by (simp add: directly_subsumes_def subsumes_coin50_100_coin50_100)
-  have merge_transitions_2: "merge_transitions pta merged_3_9 8 2 2 3 3 coin50_100 8 coin50_100 4 generator modifier True = Some merged_3_9_coin100"
+  have coin 50 100_subsumes_self: "directly_subsumes (tm pta) (tm merged_3_9) 2 coin 50 100 coin 50 100"
+    by (simp add: directly_subsumes_def subsumes_coin 50 100_coin 50 100)
+  have merge_transitions_2: "merge_transitions pta merged_3_9 8 2 2 3 3 coin 50 100 8 coin 50 100 4 generator modifier True = Some merged_3_9_coin100"
   proof-
     show ?thesis
       apply (simp add: merge_transitions_def)
-      apply (simp add: easy_merge_def coin50_100_subsumes_self)
+      apply (simp add: easy_merge_def coin 50 100_subsumes_self)
       by eval
   qed
   have arrives_5_merged_3_9_coin100: "arrives 5 merged_3_9_coin100 = 4"
   proof-
-    have ffilter: "ffilter (\<lambda>x. \<exists>a b ba. x = (5, (a, b), ba)) merged_3_9_coin100 = {|(5, (3, 4), vend_coke)|}"
+    have ffilter: "ffilter (\<lambda>x. \<exists>a b ba. x = (5, (a, b), ba)) merged_3_9_coin100 = {|(5, (3, 4), (vend coke))|}"
       apply (simp add: ffilter_def fset_both_sides Abs_fset_inverse merged_3_9_coin100_def Set.filter_def)
       apply safe
-      by (simp_all add: transitions)
+      by simp_all
     show ?thesis
       by (simp add: arrives_def ffilter)
   qed
   have arrives_9_merged_3_9_coin100: "arrives 9 merged_3_9_coin100 = 10"
   proof-
-    have ffilter: "ffilter (\<lambda>x. \<exists>a b ba. x = (9, (a, b), ba)) merged_3_9_coin100 = {|(9, (3, 10), vend_pepsi)|}"
+    have ffilter: "ffilter (\<lambda>x. \<exists>a b ba. x = (9, (a, b), ba)) merged_3_9_coin100 = {|(9, (3, 10), (vend pepsi))|}"
       apply (simp add: ffilter_def fset_both_sides Abs_fset_inverse merged_3_9_coin100_def Set.filter_def)
       apply safe
-      by (simp_all add: transitions)
+      by simp_all
     show ?thesis
       by (simp add: arrives_def ffilter)
   qed
@@ -1634,49 +1156,49 @@ proof-
     by auto
   have leaves_5_pta: "leaves 5 pta = 3"
   proof-
-    have ffilter: "ffilter (\<lambda>x. \<exists>a b ba. x = (5, (a, b), ba)) pta = {|(5, (3, 4), vend_coke)|}"
+    have ffilter: "ffilter (\<lambda>x. \<exists>a b ba. x = (5, (a, b), ba)) pta = {|(5, (3, 4), (vend coke))|}"
       apply (simp add: ffilter_def fset_both_sides Abs_fset_inverse Set.filter_def pta_def)
       apply safe
-      by (simp_all add: transitions)
+      by simp_all
     show ?thesis
       by (simp add: leaves_def ffilter)
   qed
   have leaves_9_pta: "leaves 9 pta = 9"
   proof-
-    have ffilter: "ffilter (\<lambda>x. \<exists>a b ba. x = (9, (a, b), ba)) pta = {|(9, (9, 10), vend_pepsi)|}"
+    have ffilter: "ffilter (\<lambda>x. \<exists>a b ba. x = (9, (a, b), ba)) pta = {|(9, (9, 10), (vend pepsi))|}"
       apply (simp add: ffilter_def fset_both_sides Abs_fset_inverse Set.filter_def pta_def)
       apply safe
-      by (simp_all add: transitions)
+      by simp_all
     show ?thesis
       by (simp add: leaves_def ffilter)
   qed
   have leaves_5_merged_4_10: "leaves 5 merged_4_10 = 3 \<and> arrives 5 merged_4_10 = 4"
   proof-
-    have ffilter: "ffilter (\<lambda>x. \<exists>a b ba. x = (5, (a, b), ba)) merged_4_10 = {|(5, (3, 4), vend_coke)|}"
+    have ffilter: "ffilter (\<lambda>x. \<exists>a b ba. x = (5, (a, b), ba)) merged_4_10 = {|(5, (3, 4), (vend coke))|}"
       apply (simp add: ffilter_def fset_both_sides Abs_fset_inverse Set.filter_def merged_4_10_def)
       apply safe
-      by (simp_all add: transitions)
+      by simp_all
     show ?thesis
       by (simp add: leaves_def arrives_def ffilter)
   qed
   have arrives_9_merged_4_10: "arrives 9 merged_4_10 = 4 \<and> leaves 9 merged_4_10 = 3"
   proof-
-    have ffilter: "ffilter (\<lambda>x. \<exists>a b ba. x = (9, (a, b), ba)) merged_4_10 = {|(9, (3, 4), vend_pepsi)|}"
+    have ffilter: "ffilter (\<lambda>x. \<exists>a b ba. x = (9, (a, b), ba)) merged_4_10 = {|(9, (3, 4), (vend pepsi))|}"
       apply (simp add: ffilter_def fset_both_sides Abs_fset_inverse Set.filter_def merged_4_10_def)
       apply safe
-      by (simp_all add: transitions)
+      by simp_all
     show ?thesis
       by (simp add: leaves_def arrives_def ffilter)
   qed
-  have no_direct_subsumption_vend_coke_vend_pepsi: "\<not> directly_subsumes (tm pta) (tm merged_4_10) 9 vend_coke vend_pepsi"
-    by (simp add: cant_directly_subsume no_subsumption_vend_coke_vend_pepsi)
-  have no_direct_subsumption_vend_pepsi_vend_coke: "\<not> directly_subsumes (tm pta) (tm merged_4_10) 3 vend_pepsi vend_coke"
-    by (simp add: cant_directly_subsume vend_pepsi_not_subsumes_vend_coke)
-  have merge_vend_coke_vend_pepsi: "merge_transitions pta merged_4_10 9 3 3 4 4 vend_pepsi 9 vend_coke 5 generator modifier True = Some merged_vends"
+  have no_direct_subsumption_(vend coke)_(vend pepsi): "\<not> directly_subsumes (tm pta) (tm merged_4_10) 9 (vend coke) (vend pepsi)"
+    by (simp add: cant_directly_subsume no_subsumption_(vend coke)_(vend pepsi))
+  have no_direct_subsumption_(vend pepsi)_(vend coke): "\<not> directly_subsumes (tm pta) (tm merged_4_10) 3 (vend pepsi) (vend coke)"
+    by (simp add: cant_directly_subsume (vend pepsi)_not_subsumes_(vend coke))
+  have merge_(vend coke)_(vend pepsi): "merge_transitions pta merged_4_10 9 3 3 4 4 (vend pepsi) 9 (vend coke) 5 generator modifier True = Some merged_vends"
   proof-
-    have easy_merge: "easy_merge pta merged_4_10 9 3 3 4 4 vend_pepsi 9 vend_coke 5 generator = None"
+    have easy_merge: "easy_merge pta merged_4_10 9 3 3 4 4 (vend pepsi) 9 (vend coke) 5 generator = None"
       apply (simp add: easy_merge_def generator_def)
-      by (simp add: no_direct_subsumption_vend_coke_vend_pepsi no_direct_subsumption_vend_pepsi_vend_coke)
+      by (simp add: no_direct_subsumption_(vend coke)_(vend pepsi) no_direct_subsumption_(vend pepsi)_(vend coke))
     show ?thesis
       apply (simp add: merge_transitions_def easy_merge)
       apply (simp only: modifier_def)
@@ -1697,7 +1219,7 @@ proof-
     apply (simp add: sorted_list_of_fset_def)
     apply (simp add: arrives_5_merged_3_9_coin100 arrives_9_merged_3_9_coin100 merge_states_4_10)
     apply (simp add: leaves_5_pta leaves_9_pta leaves_5_merged_4_10 arrives_9_merged_4_10)
-    by (simp add: merge_vend_coke_vend_pepsi nondeterministic_pairs_merged_vends nondeterminism_def)
+    by (simp add: merge_(vend coke)_(vend pepsi) nondeterministic_pairs_merged_vends nondeterminism_def)
 qed
 
 lemma scoring_2: "sorted_list_of_fset (score merged_vends naive_score) = [(1, 3, 5), (2, 1, 2)]"
@@ -1746,37 +1268,37 @@ proof-
     apply (simp add: outgoing_transitions_def merged_vends_def fimage_def)
     apply (simp add: naive_score_empty set_equiv)
     apply (simp add: naive_score_def fprod_def)
-    apply (simp add: transitions selectGeneral_def vend_general_def Abs_fset_inverse)
+    apply (simp add: selectGeneral_def vend_general_def Abs_fset_inverse)
     by auto
   show ?thesis
     by (simp add: scores sorted_list_of_fset_def)
 qed
 
 definition merged_1_2 :: iEFSM where
-  "merged_1_2 = {|(0, (0, 1), selectGeneral), (2, (1, 1), coin50_50),  (4, (1, 3), coin50_100), (5, (3, 4), vend_general),
-                                              (3, (1, 5), coin100_100), (6, (5, 6), vend_general)|}"
+  "merged_1_2 = {|(0, (0, 1), selectGeneral), (2, (1, 1), coin 50 50),  (4, (1, 3), coin 50 100), (5, (3, 4), vend_general),
+                                              (3, (1, 5), coin 100 100), (6, (5, 6), vend_general)|}"
 
 lemma merge_states_1_2: "merge_states 1 2 merged_vends = merged_1_2"
   by (simp add: merge_states_def merge_states_aux_def merged_vends_def merged_1_2_def)
 
 lemma nondeterministic_pairs_merged_1_2: "nondeterministic_pairs merged_1_2 = {|
-(1, (3, 1), (coin50_100, 4), coin50_50, 2),
-(1, (1, 3), (coin50_50, 2), coin50_100, 4)
+(1, (3, 1), (coin 50 100, 4), coin 50 50, 2),
+(1, (1, 3), (coin 50 50, 2), coin 50 100, 4)
 |}"
 proof-
-  have minus_1: "{|(1, coin50_50, 2), (3, coin50_100, 4), (5, coin100_100, 3)|} |-| {|(3, coin50_100, 4)|} = {|(1, coin50_50, 2), (5, coin100_100, 3)|}"
-    apply (simp add: transitions)
+  have minus_1: "{|(1, coin 50 50, 2), (3, coin 50 100, 4), (5, coin 100 100, 3)|} |-| {|(3, coin 50 100, 4)|} = {|(1, coin 50 50, 2), (5, coin 100 100, 3)|}"
+    apply simp
     by auto
-  have minus_2: "{|(1, coin50_50, 2), (3, coin50_100, 4), (5, coin100_100, 3)|} |-| {|(5, coin100_100, 3)|} = {|(1, coin50_50, 2), (3, coin50_100, 4)|}"
-    apply (simp add: transitions)
+  have minus_2: "{|(1, coin 50 50, 2), (3, coin 50 100, 4), (5, coin 100 100, 3)|} |-| {|(5, coin 100 100, 3)|} = {|(1, coin 50 50, 2), (3, coin 50 100, 4)|}"
+    apply simp
     by auto
-  have state_nondeterminism_1: "state_nondeterminism 1 {|(1, coin50_50, 2), (3, coin50_100, 4), (5, coin100_100, 3)|} = {|
-   (1, (5, 3), (coin100_100, 3), coin50_100, 4),
-   (1, (5, 1), (coin100_100, 3), coin50_50, 2),
-   (1, (3, 5), (coin50_100, 4), coin100_100, 3),
-   (1, (3, 1), (coin50_100, 4), coin50_50, 2),
-   (1, (1, 5), (coin50_50, 2), coin100_100, 3),
-   (1, (1, 3), (coin50_50, 2), coin50_100, 4)|}"
+  have state_nondeterminism_1: "state_nondeterminism 1 {|(1, coin 50 50, 2), (3, coin 50 100, 4), (5, coin 100 100, 3)|} = {|
+   (1, (5, 3), (coin 100 100, 3), coin 50 100, 4),
+   (1, (5, 1), (coin 100 100, 3), coin 50 50, 2),
+   (1, (3, 5), (coin 50 100, 4), coin 100 100, 3),
+   (1, (3, 1), (coin 50 100, 4), coin 50 50, 2),
+   (1, (1, 5), (coin 50 50, 2), coin 100 100, 3),
+   (1, (1, 3), (coin 50 50, 2), coin 50 100, 4)|}"
     apply (simp add: state_nondeterminism_def minus_1 minus_2)
     by auto
   show ?thesis
@@ -1811,13 +1333,13 @@ next
     apply (simp add: possible_steps_fst)
     apply (simp add: merged_vends_def Set.filter_def tm_def)
     apply safe
-             apply (simp_all add: transitions vend_general_def)
+             apply (simp_all add: vend_general_def)
     by force
   have possible_steps_merged_1_3_coin_vend: "\<forall>r. possible_steps (tm merged_1_3_coin) 1 r (STR ''vend'') [] = {|(4, vend_general)|}"
     apply (simp add: possible_steps_fst)
     apply (simp add: tm_def merged_1_3_coin_def Set.filter_def)
     apply safe
-           apply (simp_all add: transitions coinGeneral_def vend_general_def)
+           apply (simp_all add: coinGeneral_def vend_general_def)
     by force
   have possible_steps_merged_vends_4: "\<forall>r l i. possible_steps (tm merged_vends) 4 r l i = {||}"
     apply (simp add: possible_steps_fst)
@@ -1828,7 +1350,7 @@ next
     apply (simp add: possible_steps_fst)
     apply (simp add: merged_vends_def Set.filter_def tm_def)
     apply safe
-    by (simp_all add: transitions vend_general_def)
+    by (simp_all add: vend_general_def)
   case (Cons a t)
   then show ?case
     apply (case_tac "a= ((STR ''vend''), [])")
@@ -1860,7 +1382,7 @@ next
     apply (simp add: possible_steps_fst)
     apply (simp add: tm_def merged_1_3_coin_def Set.filter_def)
     apply safe
-           apply (simp_all add: coinGeneral_def transitions selectGeneral_2_def vend_general_def)
+           apply (simp_all add: coinGeneral_def selectGeneral_2_def vend_general_def)
     by force
   have regsimp_1: "\<forall>d. (\<lambda>a. if a = R 1 then Some d else None) = <R 1 := d>"
     apply clarify
@@ -1882,7 +1404,7 @@ next
        possible_steps (tm merged_vends) 2 r aa ba = {||}"
     apply (simp add: possible_steps_fst)
     apply (simp add: tm_def merged_vends_def Set.filter_def)
-    apply (simp add: coin50_100_def hd_input2state)
+    apply (simp add: coin 50 100_def hd_input2state)
     by (metis One_nat_def length_0_conv length_Suc_conv list.sel(1))
   case (Cons a t)
   then show ?case
@@ -1892,8 +1414,8 @@ next
          apply (simp add: nondeterministic_step_def possible_steps_merged_vends_coin50_2)
         apply (simp add: possible_steps_merged_1_3_coin_1_coin)
        apply simp
-      apply (simp add: coin50_100_def coinGeneral_def)
-     apply (simp add: coinGeneral_def coin50_100_def regsimp_1 regsimp_2)
+      apply (simp add: coin 50 100_def coinGeneral_def)
+     apply (simp add: coinGeneral_def coin 50 100_def regsimp_1 regsimp_2)
      apply (simp add: nondeterministic_simulates_trace_merged_1_3_coin_merged_vends_1_3)
     apply (case_tac a)
     apply simp
@@ -1963,7 +1485,7 @@ next
     apply (simp add: possible_steps_fst)
     apply (simp add: tm_def merged_1_3_coin_def Set.filter_def)
     apply safe
-           apply (simp_all add: coinGeneral_def vend_general_def transitions)
+           apply (simp_all add: coinGeneral_def vend_general_def)
     by force
   have regsimp_2: "\<forall>d. (\<lambda>x. if x = R 2
           then aval (snd (R 2, Plus (V (I 1)) (V (R 2))))
@@ -1976,20 +1498,20 @@ next
     apply clarify
     apply (rule ext)
     by simp
-  have possible_steps_coin_100: "\<forall>r. possible_steps (tm merged_vends) 1 r (STR ''coin'') [Num 100] = {|(5, coin100_100)|}"
+  have possible_steps_coin_100: "\<forall>r. possible_steps (tm merged_vends) 1 r (STR ''coin'') [Num 100] = {|(5, coin 100 100)|}"
     apply (simp add: possible_steps_fst)
     apply (simp add: tm_def merged_vends_def Set.filter_def)
     apply safe
-              apply (simp_all add: transitions)
+              apply simp_all
     by force
-  have possible_steps_merged_1_3_coin_coin100: "\<forall>r. possible_steps (tm merged_1_3_coin) 1 r (STR ''coin'') [Num 100] = {|(1, coinGeneral), (5, coin100_100)|}"
+  have possible_steps_merged_1_3_coin_coin100: "\<forall>r. possible_steps (tm merged_1_3_coin) 1 r (STR ''coin'') [Num 100] = {|(1, coinGeneral), (5, coin 100 100)|}"
     apply (simp add: possible_steps_fst)
     apply (simp add: tm_def merged_1_3_coin_def Set.filter_def)
     apply safe
-               apply (simp_all add: transitions coinGeneral_def vend_general_def)
+               apply (simp_all add: coinGeneral_def vend_general_def)
     apply force
     by force
-  have go_to_5: "\<forall>r. (5, coin100_100) |\<in>|
+  have go_to_5: "\<forall>r. (5, coin 100 100) |\<in>|
     possible_steps (tm merged_1_3_coin) 1 r (STR ''coin'') [Num 100]"
     by (simp add: possible_steps_merged_1_3_coin_coin100)
   have regsimp_3: "\<forall>d. (\<lambda>a. if a = R 2 then Some (Num 0) else if a = R 1 then Some d else None) = <R 1 := d, R 2 := Num 0>"
@@ -2002,7 +1524,7 @@ next
        possible_steps (tm merged_vends) 1 (\<lambda>a. if a = R 1 then Some (hd b) else None) aa ba = {||}"
     apply (simp add: possible_steps_fst)
     apply (simp add: tm_def merged_vends_def Set.filter_def)
-    apply (simp add: coin50_50_def coin100_100_def)
+    apply (simp add: coin 50 50_def coin 100 100_def)
     apply clarify
     apply simp
     apply (case_tac "bb=2")
@@ -2020,8 +1542,8 @@ next
          apply (simp add: nondeterministic_step_def possible_steps_merged_vends_coin50_1)
         apply (simp add: possible_steps_merged_1_3_coin_coin)
        apply (simp add: coinGeneral_def regsimp_2)
-      apply (simp add: coin50_50_def coinGeneral_def)
-     apply (simp add: transitions regsimp_1)
+      apply (simp add: coin 50 50_def coinGeneral_def)
+     apply (simp add: regsimp_1)
      apply (simp add: nondeterministic_simulates_trace_merged_1_3_coin_merged_vends_1_2)
     apply (case_tac "a = ((STR ''coin''), [Num 100])")
      apply simp
@@ -2029,8 +1551,8 @@ next
         apply (simp add: nondeterministic_step_def possible_steps_coin_100)
     using go_to_5 apply auto[1]
        apply simp
-      apply (simp add: coin100_100_def)
-     apply (simp add: regsimp_1 regsimp_3 coin100_100_def)
+      apply (simp add: coin 100 100_def)
+     apply (simp add: regsimp_1 regsimp_3 coin 100 100_def)
      apply (simp add: nondeterministic_simulates_trace_merged_1_3_coin_merged_vends_5_5)
     apply (case_tac a)
     apply simp
@@ -2073,7 +1595,7 @@ next
     apply (simp add: possible_steps_fst)
     apply (simp add: tm_def merged_vends_def Set.filter_def)
     apply safe
-    by (simp_all add: transitions selectGeneral_def)
+    by (simp_all add: selectGeneral_def)
   case (Cons a t)
   then show ?case
     apply (case_tac a)
@@ -2098,21 +1620,21 @@ lemma nondeterministic_simulates_merged_1_3_coin_merged_vends: "nondeterministic
   by (simp add: nondeterministic_simulates_trace_merged_1_3_coin_merged_vends_0_0)
 
 lemma nondeterministic_pairs_merged_1_3_coin: "nondeterministic_pairs merged_1_3_coin = {|
-(1, (5, 1), (coin100_100, 3), coinGeneral, 2),
-(1, (1, 5), (coinGeneral, 2), coin100_100, 3)|}"
+(1, (5, 1), (coin 100 100, 3), coinGeneral, 2),
+(1, (1, 5), (coinGeneral, 2), coin 100 100, 3)|}"
 proof-
-  have minus_1: "{|(1, coinGeneral, 2), (4, vend_general, 5), (5, coin100_100, 3)|} |-| {|(4, vend_general, 5)|} = {|(1, coinGeneral, 2), (5, coin100_100, 3)|}"
-    apply (simp add: transitions coinGeneral_def vend_general_def)
+  have minus_1: "{|(1, coinGeneral, 2), (4, vend_general, 5), (5, coin 100 100, 3)|} |-| {|(4, vend_general, 5)|} = {|(1, coinGeneral, 2), (5, coin 100 100, 3)|}"
+    apply (simp add: coinGeneral_def vend_general_def)
     by auto
-  have minus_2: "{|(1, coinGeneral, 2), (4, vend_general, 5), (5, coin100_100, 3)|} |-| {|(5, coin100_100, 3)|} = {|(1, coinGeneral, 2), (4, vend_general, 5)|}"
-    apply (simp add: transitions coinGeneral_def vend_general_def)
+  have minus_2: "{|(1, coinGeneral, 2), (4, vend_general, 5), (5, coin 100 100, 3)|} |-| {|(5, coin 100 100, 3)|} = {|(1, coinGeneral, 2), (4, vend_general, 5)|}"
+    apply (simp add: coinGeneral_def vend_general_def)
     by auto
-  have state_nondeterminism_1: "state_nondeterminism 1 {|(1, coinGeneral, 2), (4, vend_general, 5), (5, coin100_100, 3)|} = {|
-(1, (5, 4), (coin100_100, 3), vend_general, 5),
-(1, (5, 1), (coin100_100, 3), coinGeneral, 2),
-(1, (4, 5), (vend_general, 5), coin100_100, 3),
+  have state_nondeterminism_1: "state_nondeterminism 1 {|(1, coinGeneral, 2), (4, vend_general, 5), (5, coin 100 100, 3)|} = {|
+(1, (5, 4), (coin 100 100, 3), vend_general, 5),
+(1, (5, 1), (coin 100 100, 3), coinGeneral, 2),
+(1, (4, 5), (vend_general, 5), coin 100 100, 3),
 (1, (4, 1), (vend_general, 5), coinGeneral, 2),
-(1, (1, 5),(coinGeneral, 2), coin100_100, 3),
+(1, (1, 5),(coinGeneral, 2), coin 100 100, 3),
 (1, (1, 4),(coinGeneral, 2), vend_general, 5)
 |}"
     by eval
@@ -2163,13 +1685,13 @@ proof-
     by (simp_all add: choices)
 qed
 
-lemma no_direct_subsumption_coinGeneral_coin100_100:  "\<not>directly_subsumes (tm merged_vends) (tm merged_1_5) 1 coinGeneral coin100_100"
+lemma no_direct_subsumption_coinGeneral_coin 100 100:  "\<not>directly_subsumes (tm merged_vends) (tm merged_1_5) 1 coinGeneral coin 100 100"
 proof-
   have possible_steps: "\<forall>d. possible_steps (tm merged_vends) 0 Map.empty (STR ''select'') [d] = {|(1, selectGeneral)|}"
     apply (simp add: possible_steps_fst)
     apply (simp add: tm_def merged_vends_def Set.filter_def)
     apply safe
-              apply (simp_all add: transitions selectGeneral_def)
+              apply (simp_all add: selectGeneral_def)
     by force
   have possible_steps_merged_1_5: "\<forall>b. length b = 1 \<longrightarrow> possible_steps (tm merged_1_5) 0 Map.empty (STR ''select'') b = {|(1, selectGeneral_2)|}"
     apply (simp add: possible_steps_fst)
@@ -2180,9 +1702,9 @@ proof-
   have posterior_empty_selectGeneral_2: "posterior \<lbrakk>\<rbrakk> selectGeneral_2 = \<lbrakk>V (R 1) \<mapsto> Bc True, V (R 2) \<mapsto> Eq (Num 0)\<rbrakk>"
     apply (rule ext)
     by (simp add: posterior_def selectGeneral_2_def remove_input_constraints_def)
-  have medial_coin100_100: "medial \<lbrakk>V (R 1) \<mapsto> cexp.Bc True, V (R 2) \<mapsto> cexp.Eq (Num 0)\<rbrakk> (Guard coin100_100) = \<lbrakk>V (R 1) \<mapsto> cexp.Bc True, V (R 2) \<mapsto> cexp.Eq (Num 0), V (I 1) \<mapsto> Eq (Num 100)\<rbrakk>"
+  have medial_coin 100 100: "medial \<lbrakk>V (R 1) \<mapsto> cexp.Bc True, V (R 2) \<mapsto> cexp.Eq (Num 0)\<rbrakk> (Guard coin 100 100) = \<lbrakk>V (R 1) \<mapsto> cexp.Bc True, V (R 2) \<mapsto> cexp.Eq (Num 0), V (I 1) \<mapsto> Eq (Num 100)\<rbrakk>"
     apply (rule ext)
-    by (simp add: coin100_100_def)
+    by (simp add: coin 100 100_def)
   have consistent_medial: "consistent \<lbrakk>V (R 1) \<mapsto> cexp.Bc True, V (R 2) \<mapsto> cexp.Eq (Num 0), V (I 1) \<mapsto> cexp.Eq (Num 100)\<rbrakk>"
     apply (simp add: consistent_def)
     apply (rule_tac x="<R 1 := d, R 2 := Num 0, I 1 := Num 100>" in exI)
@@ -2191,13 +1713,13 @@ proof-
     apply clarify
     apply (rule ext)
     by (simp add: coinGeneral_def)
-  have subsumption_violation: " (\<exists>r i. cval (posterior (medial \<lbrakk>V (R 1) \<mapsto> cexp.Bc True, V (R 2) \<mapsto> cexp.Eq (Num 0)\<rbrakk> (Guard coin100_100)) coinGeneral r) i = Some True \<and>
-           cval (posterior \<lbrakk>V (R 1) \<mapsto> cexp.Bc True, V (R 2) \<mapsto> cexp.Eq (Num 0)\<rbrakk> coin100_100 r) i \<noteq> Some True \<and>
-           posterior \<lbrakk>V (R 1) \<mapsto> cexp.Bc True, V (R 2) \<mapsto> cexp.Eq (Num 0)\<rbrakk> coin100_100 r \<noteq> Undef)"
+  have subsumption_violation: " (\<exists>r i. cval (posterior (medial \<lbrakk>V (R 1) \<mapsto> cexp.Bc True, V (R 2) \<mapsto> cexp.Eq (Num 0)\<rbrakk> (Guard coin 100 100)) coinGeneral r) i = Some True \<and>
+           cval (posterior \<lbrakk>V (R 1) \<mapsto> cexp.Bc True, V (R 2) \<mapsto> cexp.Eq (Num 0)\<rbrakk> coin 100 100 r) i \<noteq> Some True \<and>
+           posterior \<lbrakk>V (R 1) \<mapsto> cexp.Bc True, V (R 2) \<mapsto> cexp.Eq (Num 0)\<rbrakk> coin 100 100 r \<noteq> Undef)"
     apply (rule_tac x="V (R 2)" in exI)
     apply (rule_tac x="Num 100" in exI)
-    apply (simp add: medial_coin100_100 posterior_def medial_coinGeneral Let_def consistent_medial)
-    by (simp add: remove_input_constraints_def coinGeneral_def valid_def satisfiable_def coin100_100_def)
+    apply (simp add: medial_coin 100 100 posterior_def medial_coinGeneral Let_def consistent_medial)
+    by (simp add: remove_input_constraints_def coinGeneral_def valid_def satisfiable_def coin 100 100_def)
   show ?thesis
     apply (simp add: directly_subsumes_def accepts_trace_def)
     apply standard
@@ -2214,13 +1736,13 @@ proof-
     by (simp add: subsumes_def subsumption_violation)
 qed
 
-lemma no_direct_subsumption_coin100_100_coinGeneral: "\<not> directly_subsumes (tm merged_vends) (tm merged_1_5) 1 coin100_100 coinGeneral"
+lemma no_direct_subsumption_coin 100 100_coinGeneral: "\<not> directly_subsumes (tm merged_vends) (tm merged_1_5) 1 coin 100 100 coinGeneral"
 proof-
 have possible_steps: "\<forall>d. possible_steps (tm merged_vends) 0 Map.empty (STR ''select'') [d] = {|(1, selectGeneral)|}"
     apply (simp add: possible_steps_fst)
     apply (simp add: tm_def merged_vends_def Set.filter_def)
     apply safe
-              apply (simp_all add: transitions selectGeneral_def)
+              apply (simp_all add: selectGeneral_def)
     by force
   have possible_steps_merged_1_5: "\<forall>b. length b = 1 \<longrightarrow> possible_steps (tm merged_1_5) 0 Map.empty (STR ''select'') b = {|(1, selectGeneral_2)|}"
     apply (simp add: possible_steps_fst)
@@ -2231,16 +1753,16 @@ have possible_steps: "\<forall>d. possible_steps (tm merged_vends) 0 Map.empty (
   have posterior_empty_selectGeneral_2: "posterior \<lbrakk>\<rbrakk> selectGeneral_2 = \<lbrakk>V (R 1) \<mapsto> Bc True, V (R 2) \<mapsto> Eq (Num 0)\<rbrakk>"
     apply (rule ext)
     by (simp add: posterior_def selectGeneral_2_def remove_input_constraints_def)
-  have medial_coin100_100: "medial \<lbrakk>V (R 1) \<mapsto> cexp.Bc True, V (R 2) \<mapsto> cexp.Eq (Num 0)\<rbrakk> (Guard coin100_100) = \<lbrakk>V (R 1) \<mapsto> cexp.Bc True, V (R 2) \<mapsto> cexp.Eq (Num 0), V (I 1) \<mapsto> Eq (Num 100)\<rbrakk>"
+  have medial_coin 100 100: "medial \<lbrakk>V (R 1) \<mapsto> cexp.Bc True, V (R 2) \<mapsto> cexp.Eq (Num 0)\<rbrakk> (Guard coin 100 100) = \<lbrakk>V (R 1) \<mapsto> cexp.Bc True, V (R 2) \<mapsto> cexp.Eq (Num 0), V (I 1) \<mapsto> Eq (Num 100)\<rbrakk>"
     apply (rule ext)
-    by (simp add: coin100_100_def)
+    by (simp add: coin 100 100_def)
   have medial_coinGeneral: "\<forall>c. medial c (Guard coinGeneral) = c"
     apply clarify
     apply (rule ext)
     by (simp add: coinGeneral_def)
   have subsumption_violation: "\<exists>r i. cval (medial \<lbrakk>V (R 1) \<mapsto> cexp.Bc True, V (R 2) \<mapsto> cexp.Eq (Num 0)\<rbrakk> (Guard coinGeneral) r) i = Some True \<and>
-           cval (medial \<lbrakk>V (R 1) \<mapsto> cexp.Bc True, V (R 2) \<mapsto> cexp.Eq (Num 0)\<rbrakk> (Guard coin100_100) r) i \<noteq> Some True"
-    apply (simp add: medial_coinGeneral medial_coin100_100)
+           cval (medial \<lbrakk>V (R 1) \<mapsto> cexp.Bc True, V (R 2) \<mapsto> cexp.Eq (Num 0)\<rbrakk> (Guard coin 100 100) r) i \<noteq> Some True"
+    apply (simp add: medial_coinGeneral medial_coin 100 100)
     by auto
   show ?thesis
     apply (simp add: directly_subsumes_def accepts_trace_def)
@@ -2336,7 +1858,7 @@ next
        possible_steps (tm merged_vends) 2 r aa ba = {||}"
     apply (simp add: possible_steps_fst)
     apply (simp add: tm_def merged_vends_def Set.filter_def)
-    apply (simp add: coin50_100_def hd_input2state)
+    apply (simp add: coin 50 100_def hd_input2state)
     by (metis One_nat_def length_0_conv length_Suc_conv list.sel(1))
   have coin_general_updates: "\<forall>b. (EFSM.apply_updates (Updates coinGeneral)
        (\<lambda>x. case x of I n \<Rightarrow> input2state [Num 50] 1 (I n)
@@ -2345,12 +1867,12 @@ next
     apply clarify
     apply (rule ext)
     by (simp add: coinGeneral_def)
-  have coin50_100_updates: "\<forall> b. (EFSM.apply_updates (Updates coin50_100)
+  have coin 50 100_updates: "\<forall> b. (EFSM.apply_updates (Updates coin 50 100)
        (case_vname (\<lambda>n. if n = 1 then Some (Num 50) else input2state [] (1 + 1) (I n)) (\<lambda>n. if n = 1 then Some (b) else None))
        (\<lambda>a. if a = R 1 then Some (b) else None)) = <R 1 := b>"
     apply clarify
     apply (rule ext)
-    by (simp add: coin50_100_def)
+    by (simp add: coin 50 100_def)
   case (Cons a t)
   then show ?case
     apply (case_tac "a = ((STR ''coin''), [Num 50])")
@@ -2359,8 +1881,8 @@ next
          apply (simp add: nondeterministic_step_def possible_steps_merged_vends_coin50_2)
         apply (simp add: possible_steps_merged_1_5_coin_coin)
        apply simp
-      apply (simp add: coin50_100_def coinGeneral_def)
-     apply (simp add: coin_general_updates coin50_100_updates)
+      apply (simp add: coin 50 100_def coinGeneral_def)
+     apply (simp add: coin_general_updates coin 50 100_updates)
      apply (simp add: nondeterministic_simulates_trace_merged_1_5_coin_merged_vends_1_3)
     apply (case_tac a)
     apply simp
@@ -2377,7 +1899,7 @@ next
   have possible_steps_vend: "\<forall>r. possible_steps (tm merged_vends) 5 r (STR ''vend'') [] = {|(6, vend_general)|}"
     apply (simp add: possible_steps_fst)
     apply (simp add: tm_def merged_vends_def Set.filter_def)
-    apply (simp add: transitions vend_general_def)
+    apply (simp add: vend_general_def)
     by force
   have stop: "\<forall>r aaa ba. possible_steps (tm merged_vends) 6 r aaa ba = {||}"
     apply (simp add: possible_steps_fst)
@@ -2424,7 +1946,7 @@ next
        possible_steps (tm merged_vends) 1 r aa ba = {||}"
     apply (simp add: possible_steps_fst)
     apply (simp add: tm_def merged_vends_def Set.filter_def)
-    apply (simp add: coin50_50_def coin100_100_def)
+    apply (simp add: coin 50 50_def coin 100 100_def)
     apply clarify
     apply simp
     apply (case_tac "b=2")
@@ -2441,18 +1963,18 @@ next
     apply clarify
     apply (rule ext)
     by (simp add: coinGeneral_def)
-  have updates_coin50_50: "\<forall>b. (EFSM.apply_updates (Updates coin50_50)
+  have updates_coin 50 50: "\<forall>b. (EFSM.apply_updates (Updates coin 50 50)
        (case_vname (\<lambda>n. if n = 1 then Some (Num 50) else input2state [] (1 + 1) (I n)) (\<lambda>n. if n = 1 then Some (b) else None))
        (\<lambda>a. if a = R 1 then Some (b) else None)) = <R 1 := b>"
     apply clarify
     apply (rule ext)
-    by (simp add: coin50_50_def)
-  have updates_coin100_100: "\<forall>b. (EFSM.apply_updates (Updates coin100_100)
+    by (simp add: coin 50 50_def)
+  have updates_coin 100 100: "\<forall>b. (EFSM.apply_updates (Updates coin 100 100)
        (case_vname (\<lambda>n. if n = 1 then Some (Num 100) else input2state [] (1 + 1) (I n)) (\<lambda>n. if n = 1 then Some (b) else None))
        (\<lambda>a. if a = R 1 then Some (b) else None)) = <R 1 := b>"
     apply clarify
     apply (rule ext)
-    by (simp add: coin100_100_def)
+    by (simp add: coin 100 100_def)
   have coin_general_updates_100: "\<forall>b. (EFSM.apply_updates (Updates coinGeneral)
        (\<lambda>x. case x of I n \<Rightarrow> input2state [Num 100] 1 (I n)
             | R n \<Rightarrow> if R n = R 2 then Some (Num 0) else if R n = R 1 then Some (b) else None)
@@ -2468,8 +1990,8 @@ next
          apply (simp add: nondeterministic_step_def possible_steps_merged_vends_coin50_1)
         apply (simp add: possible_steps_merged_1_5_coin_coin)
        apply simp
-      apply (simp add: coin50_50_def coinGeneral_def)
-     apply (simp only: coin_general_updates updates_coin50_50)
+      apply (simp add: coin 50 50_def coinGeneral_def)
+     apply (simp only: coin_general_updates updates_coin 50 50)
      apply (simp add: nondeterministic_simulates_trace_merged_1_5_coin_merged_vends_1_2)
     apply (case_tac "a = ((STR ''coin''), [Num 100])")
        apply simp
@@ -2477,8 +1999,8 @@ next
          apply (simp add: nondeterministic_step_def possible_steps_merged_vends_coin100)
         apply (simp add: possible_steps_merged_1_5_coin_coin)
        apply simp
-      apply (simp add: coin100_100_def coinGeneral_def)
-    apply (simp only: coin_general_updates_100 updates_coin100_100)
+      apply (simp add: coin 100 100_def coinGeneral_def)
+    apply (simp only: coin_general_updates_100 updates_coin 100 100)
     apply (simp add: nondeterministic_simulates_trace_merged_1_5_coin_merged_vends_1_5)
     apply (case_tac a)
     apply simp
@@ -2536,67 +2058,67 @@ lemma merge_1_2: "merge merged_vends 1 2 generator modifier = Some final"
 proof-
   have arrives_2_merged_1_2: "arrives 2 merged_1_2 = 1"
   proof-
-    have ffilter: "ffilter (\<lambda>x. \<exists>a b ba. x = (2, (a, b), ba)) merged_1_2 = {|(2, (1, 1), coin50_50)|}"
+    have ffilter: "ffilter (\<lambda>x. \<exists>a b ba. x = (2, (a, b), ba)) merged_1_2 = {|(2, (1, 1), coin 50 50)|}"
       apply (simp add: ffilter_def fset_both_sides Abs_fset_inverse merged_1_2_def Set.filter_def)
       apply safe
-      by (simp_all add: transitions)
+      by simp_all
     show ?thesis
       by (simp add: arrives_def ffilter)
   qed
   have arrives_4_merged_1_2: "arrives 4 merged_1_2 = 3"
   proof-
-    have ffilter: "ffilter (\<lambda>x. \<exists>a b ba. x = (4, (a, b), ba)) merged_1_2 = {|(4, (1, 3), coin50_100)|}"
+    have ffilter: "ffilter (\<lambda>x. \<exists>a b ba. x = (4, (a, b), ba)) merged_1_2 = {|(4, (1, 3), coin 50 100)|}"
       apply (simp add: ffilter_def fset_both_sides Abs_fset_inverse merged_1_2_def Set.filter_def)
       apply safe
-      by (simp_all add: transitions)
+      by simp_all
     show ?thesis
       by (simp add: arrives_def ffilter)
   qed
   have leaves_2_merged_vends: "leaves 2 merged_vends = 1"
   proof-
-    have ffilter: "ffilter (\<lambda>x. \<exists>a b ba. x = (2, (a, b), ba)) merged_vends = {|(2, (1, 2), coin50_50)|}"
+    have ffilter: "ffilter (\<lambda>x. \<exists>a b ba. x = (2, (a, b), ba)) merged_vends = {|(2, (1, 2), coin 50 50)|}"
       apply (simp add: ffilter_def fset_both_sides Abs_fset_inverse merged_vends_def Set.filter_def)
       apply safe
-      by (simp_all add: transitions)
+      by simp_all
     show ?thesis
       by (simp add: leaves_def ffilter)
   qed
   have leaves_2_merged_1_3: "(leaves 2 merged_1_3 = 1) \<and> (arrives 2 merged_1_3 = 1)"
   proof-
-    have ffilter: "ffilter (\<lambda>x. \<exists>a b ba. x = (2, (a, b), ba)) merged_1_3 = {|(2, (1, 1), coin50_50)|}"
+    have ffilter: "ffilter (\<lambda>x. \<exists>a b ba. x = (2, (a, b), ba)) merged_1_3 = {|(2, (1, 1), coin 50 50)|}"
       apply (simp add: ffilter_def fset_both_sides Abs_fset_inverse merged_1_3_def Set.filter_def)
       apply safe
-      by (simp_all add: transitions)
+      by simp_all
     show ?thesis
       by (simp add: leaves_def arrives_def ffilter)
   qed
   have leaves_4_merged_vends: "leaves 4 merged_vends = 2"
   proof-
-    have ffilter: "ffilter (\<lambda>x. \<exists>a b ba. x = (4, (a, b), ba)) merged_vends = {|(4, (2, 3), coin50_100)|}"
+    have ffilter: "ffilter (\<lambda>x. \<exists>a b ba. x = (4, (a, b), ba)) merged_vends = {|(4, (2, 3), coin 50 100)|}"
       apply (simp add: ffilter_def fset_both_sides Abs_fset_inverse merged_vends_def Set.filter_def)
       apply safe
-      by (simp_all add: transitions)
+      by simp_all
     show ?thesis
       by (simp add: leaves_def ffilter)
   qed
   have arrives_4_merged_1_3: "arrives 4 merged_1_3 = 1 \<and> leaves 4 merged_1_3 = 1"
   proof-
-    have ffilter: "ffilter (\<lambda>x. \<exists>a b ba. x = (4, (a, b), ba)) merged_1_3 = {|(4, (1, 1), coin50_100)|}"
+    have ffilter: "ffilter (\<lambda>x. \<exists>a b ba. x = (4, (a, b), ba)) merged_1_3 = {|(4, (1, 1), coin 50 100)|}"
       apply (simp add: ffilter_def fset_both_sides Abs_fset_inverse merged_1_3_def Set.filter_def)
       apply safe
-      by (simp_all add: transitions)
+      by simp_all
     show ?thesis
       by (simp add: leaves_def arrives_def ffilter)
   qed
   have merged_1_3_neq_merged_1_8: "merged_1_3 \<noteq> merged_1_8"
     apply (simp add: merged_1_3_def merged_1_8_def set_equiv)
     apply (simp only: set_nequiv_def)
-    apply (rule_tac x="(5, (3, 4), vend_coke)" in exI)
+    apply (rule_tac x="(5, (3, 4), (vend coke))" in exI)
     by simp
-  have easy_merge: "easy_merge merged_vends merged_1_3 2 1 1 1 1 coin50_100 4 coin50_50 2 generator = None"
-    apply (simp add: easy_merge_def generator_def coin50_50_cant_directly_subsume_coin50_100)
-    by (simp add: coin50_100_cant_directly_subsume_coin50_50)
-  have merge_vends: "merge_transitions merged_vends merged_1_3 2 1 1 1 1 coin50_100 4 coin50_50 2 generator modifier True = Some merged_1_3_coin"
+  have easy_merge: "easy_merge merged_vends merged_1_3 2 1 1 1 1 coin 50 100 4 coin 50 50 2 generator = None"
+    apply (simp add: easy_merge_def generator_def coin 50 50_cant_directly_subsume_coin 50 100)
+    by (simp add: coin_50_100_cant_directly_subsume_coin_50_50)
+  have merge_vends: "merge_transitions merged_vends merged_1_3 2 1 1 1 1 coin 50 100 4 coin 50 50 2 generator modifier True = Some merged_1_3_coin"
     apply (simp add: merge_transitions_def easy_merge)
     apply (simp add: modifier_def merged_1_3_neq_merged_1_8)
     by (simp add: nondeterministic_simulates_merged_1_3_coin_merged_vends)
@@ -2605,16 +2127,16 @@ proof-
     have ffilter: "ffilter (\<lambda>x. \<exists>a b ba. x = (2, (a, b), ba)) merged_1_3_coin =  {|(2, (1, 1), coinGeneral)|}"
       apply (simp add: ffilter_def merged_1_3_coin_def fset_both_sides Abs_fset_inverse Set.filter_def)
       apply safe
-      by (simp_all add: transitions)
+      by simp_all
     show ?thesis
       by (simp add: arrives_def ffilter)
   qed
   have arrives_3_merged_1_3_coin: "arrives 3 merged_1_3_coin = 5"
   proof-
-    have ffilter: "ffilter (\<lambda>x. \<exists>a b ba. x = (3, (a, b), ba)) merged_1_3_coin = {|(3, (1, 5), coin100_100)|}"
+    have ffilter: "ffilter (\<lambda>x. \<exists>a b ba. x = (3, (a, b), ba)) merged_1_3_coin = {|(3, (1, 5), coin 100 100)|}"
       apply (simp add: ffilter_def merged_1_3_coin_def fset_both_sides Abs_fset_inverse Set.filter_def)
       apply safe
-      by (simp_all add: transitions)
+      by simp_all
     show ?thesis
       by (simp add: arrives_def ffilter)
   qed
@@ -2622,10 +2144,10 @@ proof-
     by (simp add: merge_states_def merge_states_aux_def merged_1_3_coin_def merged_1_5_def)
   have leaves_3_merged_vends: "leaves 3 merged_vends = 1"
   proof-
-    have ffilter: "ffilter (\<lambda>x. \<exists>a b ba. x = (3, (a, b), ba)) merged_vends = {|(3, (1, 5), coin100_100)|}"
+    have ffilter: "ffilter (\<lambda>x. \<exists>a b ba. x = (3, (a, b), ba)) merged_vends = {|(3, (1, 5), coin 100 100)|}"
       apply (simp add: ffilter_def merged_vends_def Abs_fset_inverse fset_both_sides Set.filter_def)
       apply safe
-      by (simp_all add: transitions)
+      by simp_all
     show ?thesis
       by (simp add: leaves_def ffilter)
   qed
@@ -2640,24 +2162,24 @@ proof-
   qed
   have arrives_3_merged_1_5: "arrives 3 merged_1_5 = 1 \<and> leaves 3 merged_1_5 = 1"
   proof-
-    have ffilter: "ffilter (\<lambda>x. \<exists>a b ba. x = (3, (a, b), ba)) merged_1_5 = {|(3, (1, 1), coin100_100)|}"
+    have ffilter: "ffilter (\<lambda>x. \<exists>a b ba. x = (3, (a, b), ba)) merged_1_5 = {|(3, (1, 1), coin 100 100)|}"
       apply (simp add: ffilter_def merged_1_5_def Abs_fset_inverse fset_both_sides Set.filter_def)
       apply safe
       by (simp_all add: coinGeneral_def)
     show ?thesis
       by (simp add: leaves_def arrives_def ffilter)
   qed
-  have easy_merge_1_5: "easy_merge merged_vends merged_1_5 1 1 1 1 1 coin100_100 3 coinGeneral 2 generator = None"
+  have easy_merge_1_5: "easy_merge merged_vends merged_1_5 1 1 1 1 1 coin 100 100 3 coinGeneral 2 generator = None"
   proof-
-    have ffilter: "ffilter (\<lambda>x. snd x \<noteq> ((1, 1), coin100_100) \<and> snd x \<noteq> ((1, 1), coinGeneral)) merged_1_5 = {|(0, (0, 1), selectGeneral_2), (5, (1, 4), vend_general),
+    have ffilter: "ffilter (\<lambda>x. snd x \<noteq> ((1, 1), coin 100 100) \<and> snd x \<noteq> ((1, 1), coinGeneral)) merged_1_5 = {|(0, (0, 1), selectGeneral_2), (5, (1, 4), vend_general),
       (6, (1, 6), vend_general)|}"
       apply (simp add: ffilter_def fset_both_sides Abs_fset_inverse merged_1_5_def Set.filter_def)
       by auto
     show ?thesis
-      apply (simp add: easy_merge_def no_direct_subsumption_coinGeneral_coin100_100 no_direct_subsumption_coin100_100_coinGeneral)
+      apply (simp add: easy_merge_def no_direct_subsumption_coinGeneral_coin 100 100 no_direct_subsumption_coin 100 100_coinGeneral)
       by (simp add: replace_transition_def ffilter merged_1_5_coin_def generator_def)
   qed
-  have merge_coins: "merge_transitions merged_vends merged_1_5 1 1 1 1 1 coin100_100 3 coinGeneral 2 generator modifier True = Some merged_1_5_coin"
+  have merge_coins: "merge_transitions merged_vends merged_1_5 1 1 1 1 1 coin 100 100 3 coinGeneral 2 generator modifier True = Some merged_1_5_coin"
     apply (simp add: merge_transitions_def easy_merge_1_5)
     apply (simp add: modifier_def)
     apply (simp add: nondeterministic_simulates_def nondeterministic_simulates_trace_merged_1_5_coin_merged_vends_0_0)
@@ -2760,10 +2282,9 @@ proof-
     by auto
 qed
 
-lemma "learn traces naive_score generator modifier = (tm final)"
-  apply (simp add: learn_def build_pta scoring_1 merge_1_8 merge_1_7)
-  apply (simp add: scoring_2 merge_1_2)
-  by (simp add: score_final sorted_list_of_fset_def)
+lemma "learn traces naive_score generator (heuristic_1 traces) = (tm final)"
+  apply (simp add: learn_def build_pta scoring_1 merge_1_8)
+
 
 (* value "iefsm2dot pta" *)
 (* value "iefsm2dot merged_1_8" *)
