formal/inference/General_Subsumption.thy
@@ -1,38 +1,10 @@
 theory General_Subsumption
-imports "../Contexts" Trace_Matches
+imports "../Contexts" Trace_Matches Code_Generation
 begin
 
 lemma ctx_simp: "(\<lambda>r. and (if r = V (I i) then snd (V (I i), cexp.Eq s) else cexp.Bc True) (\<lbrakk>\<rbrakk> r)) = \<lbrakk>V (I i) \<mapsto> Eq s\<rbrakk>"
   apply (rule ext)
   by simp
-
-lemma generalise_subsumption: "subsumes \<lbrakk>\<rbrakk> \<lparr>Label=l, Arity=a, Guard=[], Outputs=[], Updates=[(R r, (V (I i)))]\<rparr> 
-                  \<lparr>Label=l, Arity=a, Guard=[GExp.Eq (V (I i)) (L s)], Outputs=[], Updates=[]\<rparr>"
-  apply (simp add: subsumes_def)
-  apply standard
-   apply clarify
-   apply (case_tac "cval (\<lbrakk>\<rbrakk> r) ia")
-    apply simp
-   apply simp
-
-  apply standard
-   apply clarify
-   apply (simp add: posterior_def Let_def ctx_simp)
-   apply (case_tac "consistent \<lbrakk>V (I i) \<mapsto> cexp.Eq s\<rbrakk>")
-    apply (simp add: remove_input_constraints_def)
-    apply (case_tac "constrains_an_input ra")
-     apply simp
-    apply simp
-    apply (case_tac "ra = V (R r)")
-     apply simp
-    apply (case_tac "ra = V (I i)")
-     apply simp
-    apply simp
-   apply simp
-   apply (simp add: posterior_def Let_def ctx_simp)
-  apply standard
-   apply (simp add: consistent_def remove_input_constraints_def consistent_empty_4)
-  by (simp add: inconsistent_false)
 
 lemma incoming_transition_alt_def: "incoming_transition_to e n = (\<exists>t from. ((from, n), t) |\<in>| e)"
   apply (simp add: incoming_transition_to_def)
@@ -100,47 +72,6 @@ next
     by auto
 qed
 
-
-lemma "\<not> incoming_transition_to t 0 \<Longrightarrow> directly_subsumes t t' 0 \<lparr>Label=l, Arity=a, Guard=[], Outputs=[], Updates=[(R r, (V (I i)))]\<rparr> 
-                  \<lparr>Label=l, Arity=a, Guard=[GExp.Eq (V (I i)) (L s)], Outputs=[], Updates=[]\<rparr>"
-  apply (simp add: directly_subsumes_def anterior_context_no_return_to_zero)
-  apply (simp add: generalise_subsumption)
-  using generalise_subsumption
-  by blast
-
-lemma "subsumes \<lbrakk>\<rbrakk> (remove_guard_add_update \<lparr>Label=l, Arity=a, Guard=[GExp.Eq (V (I i)) (L s)], Outputs=[], Updates=[]\<rparr> i r)
-                  \<lparr>Label=l, Arity=a, Guard=[GExp.Eq (V (I i)) (L s)], Outputs=[], Updates=[]\<rparr>"
-  apply (simp add: subsumes_def)
-  apply safe
-          apply (simp add: remove_guard_add_update_def)
-         apply (simp add: remove_guard_add_update_def)
-        apply (simp add: remove_guard_add_update_def)
-       apply (simp add: remove_guard_add_update_def)
-      apply (case_tac "cval (\<lbrakk>\<rbrakk> ra) ia")
-       apply simp
-      apply (simp add: remove_guard_add_update_def)
-     apply (simp add: remove_guard_add_update_def)
-    apply (simp add: remove_guard_add_update_def)
-   apply (simp add: remove_guard_add_update_def)
-   apply (simp add: posterior_def Let_def ctx_simp)
-   apply (case_tac "consistent \<lbrakk>V (I i) \<mapsto> cexp.Eq s\<rbrakk>")
-    apply (simp add: remove_input_constraints_def)
-    apply (case_tac "constrains_an_input ra")
-     apply simp
-    apply simp
-    apply (case_tac "ra = V (R r)")
-     apply simp
-    apply (case_tac "ra = V (I i)")
-     apply simp
-    apply simp
-   apply simp
-  apply (simp add: remove_guard_add_update_def)
-  apply (simp add: posterior_def Let_def ctx_simp)
-  apply (case_tac "consistent \<lbrakk>V (I i) \<mapsto> cexp.Eq s\<rbrakk>")
-   apply (simp add: remove_input_constraints_def consistent_def)
-   apply auto[1]
-  by (simp add: inconsistent_false)
-
 lemma inconsistent_c: "\<not>consistent c \<Longrightarrow> \<not>consistent (\<lambda>r. and (if r = V (I i) then snd (V (I i), cexp.Eq s) else cexp.Bc True) (c r))"
 proof-
   assume premise: "\<not> consistent c"
@@ -194,10 +125,10 @@ lemma test2: "consistent (\<lambda>r. and (if r = V (I i) then snd (V (I i), cex
   using inconsistent_c
   by auto
 
-lemma "c (V (R ri)) = Undef \<Longrightarrow> 
-       c (V (I i)) = Bc True \<Longrightarrow> 
-       subsumes c (remove_guard_add_update \<lparr>Label=l, Arity=a, Guard=[GExp.Eq (V (I i)) (L v)], Outputs=[], Updates=[]\<rparr> i ri)
-                                           \<lparr>Label=l, Arity=a, Guard=[GExp.Eq (V (I i)) (L v)], Outputs=[], Updates=[]\<rparr>"
+lemma generalise_subsumption: "c (V (R ri)) = Undef \<Longrightarrow> 
+                               c (V (I i)) = Bc True \<Longrightarrow> 
+                               subsumes c (remove_guard_add_update \<lparr>Label=l, Arity=a, Guard=[GExp.Eq (V (I i)) (L v)], Outputs=[], Updates=[]\<rparr> i ri)
+                                                                   \<lparr>Label=l, Arity=a, Guard=[GExp.Eq (V (I i)) (L v)], Outputs=[], Updates=[]\<rparr>"
   apply (simp add: subsumes_def)
   apply safe
           apply (simp add: remove_guard_add_update_def)
@@ -242,6 +173,29 @@ lemma "c (V (R ri)) = Undef \<Longrightarrow>
   apply clarify
   by (metis (full_types))
 
+lemma empty_variable_constraints: "\<lbrakk>\<rbrakk> (V (R ri)) = Undef \<and> \<lbrakk>\<rbrakk> (V (I i)) = Bc True"
+  by simp
+
+lemma remove_guard_add_update:  "\<lparr>Label=l, Arity=a, Guard=[], Outputs=[], Updates=[(R r, (V (I i)))]\<rparr> = remove_guard_add_update \<lparr>Label=l, Arity=a, Guard=[GExp.Eq (V (I i)) (L s)], Outputs=[], Updates=[]\<rparr> i r"
+  by (simp add: remove_guard_add_update_def)
+
+lemma generalise_subsumption_empty: "subsumes \<lbrakk>\<rbrakk> \<lparr>Label=l, Arity=a, Guard=[], Outputs=[], Updates=[(R r, (V (I i)))]\<rparr> 
+                  \<lparr>Label=l, Arity=a, Guard=[GExp.Eq (V (I i)) (L s)], Outputs=[], Updates=[]\<rparr>"
+  using remove_guard_add_update empty_variable_constraints generalise_subsumption
+  by simp
+
+lemma "subsumes \<lbrakk>\<rbrakk> (remove_guard_add_update \<lparr>Label=l, Arity=a, Guard=[GExp.Eq (V (I i)) (L s)], Outputs=[], Updates=[]\<rparr> i r)
+                  \<lparr>Label=l, Arity=a, Guard=[GExp.Eq (V (I i)) (L s)], Outputs=[], Updates=[]\<rparr>"
+  using remove_guard_add_update empty_variable_constraints generalise_subsumption
+  by simp
+
+lemma "\<not> incoming_transition_to t 0 \<Longrightarrow> directly_subsumes t t' 0 \<lparr>Label=l, Arity=a, Guard=[], Outputs=[], Updates=[(R r, (V (I i)))]\<rparr> 
+                                                                 \<lparr>Label=l, Arity=a, Guard=[GExp.Eq (V (I i)) (L s)], Outputs=[], Updates=[]\<rparr>"
+  apply (simp add: directly_subsumes_def anterior_context_no_return_to_zero)
+  apply (simp add: generalise_subsumption_empty)
+  using generalise_subsumption_empty
+  by blast
+
 lemma posterior_input: "(posterior \<lbrakk>\<rbrakk> aaa) (V(I i)) = Bc False \<Longrightarrow> (posterior \<lbrakk>\<rbrakk> aaa) = (\<lambda>x. Bc False)"
   apply (simp add: posterior_def Let_def)
   apply (case_tac "consistent (medial \<lbrakk>\<rbrakk> (Guard aaa))")
@@ -265,39 +219,6 @@ lemma gval_and_false: "gval (cexp2gexp r (and (cexp.Bc False) c)) s \<noteq> Som
   apply (case_tac "gval (cexp2gexp r x72) s")
   by auto
 
-lemma context_equiv_conjoin_false: "context_equiv (Contexts.conjoin (\<lambda>r. cexp.Bc False) c) (\<lambda>r. cexp.Bc False)"
-  apply (simp add: context_equiv_def cexp_equiv_def)
-  apply clarify
-  apply standard
-   apply clarify
-  sorry
-
-declare conjoin.simps [simp del]
-
-lemma context_equiv_false_medial: "\<And>c. context_equiv c (\<lambda>x. Bc False) \<Longrightarrow> context_equiv (medial c g) (\<lambda>x. Bc False)"
-proof(induct g)
-  case Nil
-  then show ?case
-    by simp
-next
-  case (Cons a g)
-  then show ?case
-    apply (case_tac a)
-        apply (case_tac x1)
-         apply (simp add: conjoin.simps)
-        apply simp
-        apply (simp add: context_equiv_conjoin_false)
-    sorry
-
-qed
-declare conjoin.simps [simp]
-
-lemma not_cexp_equiv_lt_false: "\<not>cexp_equiv (cexp.Lt s) (cexp.Bc False)"
-  apply (case_tac s)
-  apply (simp add: cexp_equiv_def)
-  apply (metis MaybeBoolInt.simps(1) MaybeBoolInt.simps(3) lt_ex option.inject)
-  by (simp add: cexp_equiv_def)
-
 lemma not_cexp_equiv_gt_false: "\<not>cexp_equiv (cexp.Gt x5) (cexp.Bc False)"
   apply (case_tac x5)
   apply (simp add: cexp_equiv_def)
@@ -307,62 +228,8 @@ lemma not_cexp_equiv_gt_false: "\<not>cexp_equiv (cexp.Gt x5) (cexp.Bc False)"
 lemma maybe_double_negation: "maybe_not (maybe_not x) = x"
   by (simp add: option.case_eq_if)
 
-lemma maybe_negate: "(\<forall>i. maybe_not (cval x i) = Some False) = (\<forall>i. (cval x i) = Some True)"
-proof(induct x)
-  case Undef
-  then show ?case
-    by simp
-next
-  case (Bc x)
-  then show ?case
-    apply (case_tac x)
-    by auto
-next
-  case (Eq x)
-  then show ?case
-    by simp
-next
-  case (Lt x)
-  then show ?case
-    apply simp
-    by (metis MaybeBoolInt.simps(3) option.case_eq_if option.simps(3))
-next
-  case (Gt x)
-  then show ?case
-    apply simp
-    by (metis MaybeBoolInt.simps(3) option.case_eq_if option.simps(3))
-next
-  case (Not x)
-  then show ?case
-    apply (simp add: maybe_double_negation)
-    by (metis cval.simps(2) cval.simps(6) cval_double_negation false_not_true)
-next
-  case (And x1 x2)
-  then show ?case
-    apply safe
-           apply simp+
-         apply (case_tac "cval x2 ib")
-          apply (metis option.case_eq_if option.distinct(1))
-         apply simp
-         apply (metis option.inject option.simps(5))
-        apply simp+
-       apply (case_tac "cval x1 ib")
-        apply simp
-        apply (metis option.distinct(1) option.simps(4))
-       apply simp
-       apply (metis (no_types, lifting) cval.simps(2) option.case_eq_if option.sel true_or_none_not_false)
-      apply simp+
-     apply (case_tac "cval x1 id")
-      apply simp
-      apply (metis option.case_eq_if option.simps(3))
-     apply simp
-     apply (case_tac "cval x2 id")
-      apply simp
-      apply (metis (no_types, lifting) option.case_eq_if option.simps(3))
-     apply simp
-     apply (smt is_none_code(2) option.simps(4) option.split_sel_asm true_or_none_not_false)
-    by simp
-qed
+lemma maybe_negate: "(maybe_not c = Some False) = (c = Some True)"
+  by (metis (mono_tags, lifting) maybe_double_negation option.simps(5))
 
 lemma maybe_not_values: "(maybe_not c \<noteq> Some False) = (maybe_not c = Some True \<or> maybe_not c = None)"
   by auto
@@ -373,116 +240,37 @@ lemma maybe_not_c: "(maybe_not c \<noteq> Some False) = (c = None \<or> c = Some
 lemma cval_values: "(cval x i \<noteq> Some False) = (cval x i = Some True \<or> cval x i = None)"
   by auto
 
-lemma remove_maybe_not: "(maybe_not (cval x6 i) \<noteq> Some False) = (cval x6 i \<noteq> Some True)"
+lemma remove_maybe_not: "(maybe_not c \<noteq> Some False) = (c \<noteq> Some True)"
   using cval_values maybe_not_c by auto
 
 lemma x_nec_not_x: "x \<noteq> cexp.Not x"
   apply (induct_tac x)
   by auto
 
-fun "and2" :: "cexp \<Rightarrow> cexp \<Rightarrow> cexp" where
-  "and2 (Bc True) x = x" |
-  "and2 x (Bc True) = x" |
-  "and2 Undef Undef = Undef" |
-  "and2 Undef c' = And Undef c'" |
-  "and2 c Undef = And c Undef" |
-  "and2 (Bc False) x = x" |
-  "and2 x (Bc False) = x" |
-  "and2 c c' = (if c = c' then c else And c c')"
+lemma filter_not_f_a: " \<not> f a \<Longrightarrow> filter f g = filter f (a#g)"
+  by simp
 
-lemma "cexp_equiv (and2 x y) (And x y)"
-proof(induct x)
-case Undef
-  then show ?case
-    apply (induct_tac y)
-          apply simp
-    unfolding cexp_equiv_def
-next
-  case (Bc x)
-  then show ?case sorry
-next
-  case (Eq x)
-then show ?case sorry
-next
-  case (Lt x)
-  then show ?case sorry
-next
-  case (Gt x)
-  then show ?case sorry
-next
-  case (Not x)
-  then show ?case sorry
-next
-  case (And x1 x2)
-  then show ?case sorry
-qed
+lemma and_false_not_undef: "and (cexp.Bc False) c \<noteq> Undef"
+  apply (induct_tac c)
+        apply simp
+       apply (case_tac x)
+  by auto
 
-lemma "\<not>consistent (medial (\<lambda>x. cexp.Bc False) g)"
-  apply (simp add: consistent_def)
+lemma and_And_false: "x \<noteq> cexp.Bc True \<and> x \<noteq> Bc False \<Longrightarrow> and (Bc False) x = And (Bc False) x"
+  apply (case_tac x)
+  by auto
+
+lemma inconsistant_conjoin_false: "\<not>consistent (Contexts.conjoin (\<lambda>r. cexp.Bc False) c)"
+  apply (simp add: consistent_def and_false_not_undef)
   apply clarify
   apply (rule_tac x=x in exI)
-  apply standard
-  using context_equiv_false_medial context_equiv_reflexive context_equiv_undef apply blast
-  
-
-lemma "posterior (\<lambda>x. cexp.Bc False) aaa = (\<lambda>x. Bc False)"
-  apply (simp add: posterior_def Let_def)
-
-lemma "\<forall>s r. posterior_sequence (\<lambda>x. cexp.Bc False) e s r t = (\<lambda>x. Bc False)"
-proof(induct t)
-  case Nil
-  then show ?case
-    by simp
-next
-  case (Cons a t)
-  then show ?case
-    apply clarify
-    apply simp
-    apply (case_tac "step e s r (fst a) (snd a)")
-     apply simp
-    apply simp
-    apply (case_tac aa)
-    apply simp
-
-
-qed
-
-lemma "(anterior_context e t) (V(I i)) \<noteq> Bc True \<Longrightarrow> (anterior_context e t) (V(I i)) = Bc False"
-proof(induct t)
-  case Nil
-  then show ?case
-    by (simp add: anterior_context_def)
-next
-  case (Cons a t)
-  then show ?case
-    apply (simp add: anterior_context_def)
-    apply (case_tac "step e 0 Map.empty (fst a) (snd a)")
-     apply simp
-    apply simp
-    apply (case_tac aa)
-    apply clarify
-    apply simp
-    apply (case_tac "(posterior \<lbrakk>\<rbrakk> aaa) = (\<lambda>x. Bc False)")
-     apply simp
-
-qed
-
-lemma "accepts_trace e t \<Longrightarrow> (anterior_context e t) (V(I i)) = Bc True"
-proof(induct t)
-case Nil
-  then show ?case
-    by (simp add: anterior_context_def)
-next
-  case (Cons a t)
-  then show ?case
-    apply (simp add: anterior_context_def)
-    apply (case_tac "step e 0 Map.empty (fst a) (snd a)")
-     apply simp
-    apply simp
-    apply (case_tac aa)
-    apply clarify
-    apply simp
-
-qed
+  apply (case_tac "c x = Bc True")
+   apply simp
+  apply (case_tac "c x = Bc False")
+   apply simp
+  apply (simp add: and_And_false)
+  apply (case_tac "gval (cexp2gexp x (c x)) s")
+   apply simp
+  by simp
 
 end
